<?xml version="1.0"?>
<rdf:RDF xmlns="https://w3id.org/transmodel/journeys#"
     xml:base="https://w3id.org/transmodel/journeys"
     xmlns:cc="http://creativecommons.org/ns#"
     xmlns:dc="http://purl.org/dc/elements/1.1/"
     xmlns:geo="https://www.w3.org/2003/01/geo/"
     xmlns:owl="http://www.w3.org/2002/07/owl#"
     xmlns:rdf="http://www.w3.org/1999/02/22-rdf-syntax-ns#"
     xmlns:xml="http://www.w3.org/XML/1998/namespace"
     xmlns:xsd="http://www.w3.org/2001/XMLSchema#"
     xmlns:rdfs="http://www.w3.org/2000/01/rdf-schema#"
     xmlns:vann="http://purl.org/vocab/vann/"
     xmlns:tmfac="https://w3id.org/transmodel/facilities#"
     xmlns:tmkos="https://w3id.org/transmodel/kos/"
     xmlns:tmorg="https://w3id.org/transmodel/organisations#"
     xmlns:tmfare="https://w3id.org/transmodel/fares#"
     xmlns:tmkosorg="https://w3id.org/transmodel/kos/organisations/"
     xmlns:tmcommons="https://w3id.org/transmodel/commons#"
     xmlns:tmjourney="https://w3id.org/transmodel/journeys#"
     xmlns:tmkosfare="https://w3id.org/transmodel/kos/fares/"
     xmlns:tmkoscommons="https://w3id.org/transmodel/kos/commons/"
     xmlns:tmkosjourney="https://w3id.org/transmodel/kos/journeys/"
     xmlns:tmkosfacility="https://w3id.org/transmodel/kos/facilities/">
    <owl:Ontology rdf:about="https://w3id.org/transmodel/journeys#">
        <owl:versionIRI rdf:resource="https://w3id.org/transmodel/journeys/0.3"/>
        <cc:license rdf:resource="http://creativecommons.org/licenses/by/4.0/"/>
        <dc:creator>Adolfo Antón Bravo (Ontology Engineering Group - Universidad Politécnica de Madrid)</dc:creator>
        <dc:creator>Oscar Corcho (Ontology Engineering Group - Universidad Politécnica de Madrid)</dc:creator>
        <dc:date>2019-11-22</dc:date>
        <dc:description xml:lang="en">Module of the Transmodel Ontology focused on journeys. This ontology provides support to the NeTEx model. Visit https://github.com/oeg-upm/transmodel-ontology</dc:description>
        <dc:identifier>https://w3id.org/transmodel/journeys</dc:identifier>
        <dc:rights>Creative Commons Attribution 4.0 International (CC BY 4.0)</dc:rights>
        <dc:title xml:lang="en">Transmodel Ontology - Journeys</dc:title>
        <vann:preferredNamespaceUri rdf:resource="https://w3id.org/transmodel/journeys#"/>
        <rdfs:comment xml:lang="en">Module of the Transmodel Ontology focused on facilities. This ontology provides support to the NeTEx model. Visit https://github.com/oeg-upm/transmodel-ontology</rdfs:comment>
        <rdfs:label xml:lang="en">Transmodel Ontology - Journeys</rdfs:label>
        <rdfs:seeAlso xml:lang="en">https://github.com/oeg-upm/transmodel-ontology</rdfs:seeAlso>
        <owl:versionInfo xml:lang="en">This is the initial version of the module on Journeys, after considering the UML models and XSD descriptions of Transmodel and NeTEx</owl:versionInfo>
    </owl:Ontology>
    


    <!-- 
    ///////////////////////////////////////////////////////////////////////////////////////
    //
    // Annotation properties
    //
    ///////////////////////////////////////////////////////////////////////////////////////
     -->

    


    <!-- http://creativecommons.org/ns#license -->

    <owl:AnnotationProperty rdf:about="http://creativecommons.org/ns#license"/>
    


    <!-- http://purl.org/dc/elements/1.1/creator -->

    <owl:AnnotationProperty rdf:about="http://purl.org/dc/elements/1.1/creator"/>
    


    <!-- http://purl.org/dc/elements/1.1/date -->

    <owl:AnnotationProperty rdf:about="http://purl.org/dc/elements/1.1/date"/>
    


    <!-- http://purl.org/dc/elements/1.1/description -->

    <owl:AnnotationProperty rdf:about="http://purl.org/dc/elements/1.1/description"/>
    


    <!-- http://purl.org/dc/elements/1.1/identifier -->

    <owl:AnnotationProperty rdf:about="http://purl.org/dc/elements/1.1/identifier"/>
    


    <!-- http://purl.org/dc/elements/1.1/rights -->

    <owl:AnnotationProperty rdf:about="http://purl.org/dc/elements/1.1/rights"/>
    


    <!-- http://purl.org/dc/elements/1.1/title -->

    <owl:AnnotationProperty rdf:about="http://purl.org/dc/elements/1.1/title"/>
    


    <!-- http://purl.org/vocab/vann/preferredNamespaceUri -->

    <owl:AnnotationProperty rdf:about="http://purl.org/vocab/vann/preferredNamespaceUri"/>
    


    <!-- https://w3id.org/transmodel/journeys#author -->

    <owl:AnnotationProperty rdf:about="https://w3id.org/transmodel/journeys#author"/>
    


    <!-- https://w3id.org/transmodel/journeys#creator -->

    <owl:AnnotationProperty rdf:about="https://w3id.org/transmodel/journeys#creator"/>
    


    <!-- https://w3id.org/transmodel/journeys#description -->

    <owl:AnnotationProperty rdf:about="https://w3id.org/transmodel/journeys#description">
        <rdfs:range rdf:resource="http://www.w3.org/2000/01/rdf-schema#Literal"/>
        <rdfs:domain rdf:resource="https://w3id.org/transmodel/journeys#MeetingPointService"/>
    </owl:AnnotationProperty>
    


    <!-- https://w3id.org/transmodel/journeys#mbox -->

    <owl:AnnotationProperty rdf:about="https://w3id.org/transmodel/journeys#mbox"/>
    


    <!-- https://w3id.org/transmodel/journeys#name -->

    <owl:AnnotationProperty rdf:about="https://w3id.org/transmodel/journeys#name">
        <rdfs:range rdf:resource="http://www.w3.org/2000/01/rdf-schema#Literal"/>
    </owl:AnnotationProperty>
    


    <!-- 
    ///////////////////////////////////////////////////////////////////////////////////////
    //
    // Datatypes
    //
    ///////////////////////////////////////////////////////////////////////////////////////
     -->

    


    <!-- http://www.w3.org/2000/01/rdf-schema#range -->

    <rdfs:Datatype rdf:about="http://www.w3.org/2000/01/rdf-schema#range"/>
    


    <!-- http://www.w3.org/2001/XMLSchema#duration -->

    <rdfs:Datatype rdf:about="http://www.w3.org/2001/XMLSchema#duration"/>
    


    <!-- http://www.w3.org/2001/XMLSchema#time -->

    <rdfs:Datatype rdf:about="http://www.w3.org/2001/XMLSchema#time"/>
    


    <!-- 
    ///////////////////////////////////////////////////////////////////////////////////////
    //
    // Object Properties
    //
    ///////////////////////////////////////////////////////////////////////////////////////
     -->

    


    <!-- http://www.w3.org/2004/02/skos/core#inScheme -->

    <owl:ObjectProperty rdf:about="http://www.w3.org/2004/02/skos/core#inScheme"/>
    


    <!-- https://w3id.org/transmodel/commons#at -->

    <owl:ObjectProperty rdf:about="https://w3id.org/transmodel/commons#at">
        <rdfs:subPropertyOf rdf:resource="http://www.w3.org/2002/07/owl#topObjectProperty"/>
    </owl:ObjectProperty>
    


    <!-- https://w3id.org/transmodel/commons#in -->

    <owl:ObjectProperty rdf:about="https://w3id.org/transmodel/commons#in">
        <rdfs:subPropertyOf rdf:resource="http://www.w3.org/2002/07/owl#topObjectProperty"/>
    </owl:ObjectProperty>
    


    <!-- https://w3id.org/transmodel/facilities#journeyPatternAdvertisedFor -->

    <owl:ObjectProperty rdf:about="https://w3id.org/transmodel/facilities#journeyPatternAdvertisedFor">
        <rdfs:subPropertyOf rdf:resource="https://w3id.org/transmodel/journeys#PROPS-TO-REVIEW"/>
        <rdfs:domain rdf:resource="https://w3id.org/transmodel/facilities#JourneyPattern"/>
        <rdfs:range rdf:resource="https://w3id.org/transmodel/journeys#DestinationDisplay"/>
        <rdfs:comment xml:lang="en">A Journey Pattern is advertised in a Destination Display</rdfs:comment>
        <rdfs:comment xml:lang="en">TODO: change to aViewOf</rdfs:comment>
        <rdfs:label xml:lang="en">journey Pattern Advertised For</rdfs:label>
    </owl:ObjectProperty>
    


    <!-- https://w3id.org/transmodel/journeys#PROPS-TO-REVIEW -->

    <owl:ObjectProperty rdf:about="https://w3id.org/transmodel/journeys#PROPS-TO-REVIEW"/>
    


    <!-- https://w3id.org/transmodel/journeys#aViewOf -->

    <owl:ObjectProperty rdf:about="https://w3id.org/transmodel/journeys#aViewOf">
        <rdfs:subPropertyOf rdf:resource="http://www.w3.org/2002/07/owl#topObjectProperty"/>
        <owl:inverseOf rdf:resource="https://w3id.org/transmodel/journeys#viewedAs"/>
        <rdfs:domain rdf:resource="https://w3id.org/transmodel/journeys#Point"/>
        <rdfs:range rdf:resource="https://w3id.org/transmodel/journeys#PointInLinkSequence"/>
        <rdfs:comment xml:lang="en">This property allows relating a Point with the Points in Link Sequence where it appears</rdfs:comment>
        <rdfs:label xml:lang="en">a View Of</rdfs:label>
    </owl:ObjectProperty>
    


    <!-- https://w3id.org/transmodel/journeys#accessMode -->

    <owl:ObjectProperty rdf:about="https://w3id.org/transmodel/journeys#accessMode">
        <rdfs:subPropertyOf rdf:resource="https://w3id.org/transmodel/journeys#PROPS-TO-REVIEW"/>
        <rdfs:range rdf:resource="https://w3id.org/transmodel/journeys#AccessMode"/>
        <rdfs:label xml:lang="en">accessMode</rdfs:label>
    </owl:ObjectProperty>
    


    <!-- https://w3id.org/transmodel/journeys#accessPTS -->

    <owl:ObjectProperty rdf:about="https://w3id.org/transmodel/journeys#accessPTS">
        <rdfs:subPropertyOf rdf:resource="https://w3id.org/transmodel/journeys#PROPS-TO-REVIEW"/>
        <rdfs:range rdf:resource="https://w3id.org/transmodel/journeys#Access"/>
        <rdfs:comment xml:lang="en">The physical spatial possibility for a passenger to access or leave the Public Transport System. The link may be used during a Trip for :
- The walking movement of the Passenger from a Place (Origin of the Trip) to a ScheduledStopPoint (origin of the Public Transport Trip) or;
- The walking movement of the Passenger from a Scheduled Stop Point (destination of the Public Transport Trip) to a Place (destination of the Trip)</rdfs:comment>
        <rdfs:label xml:lang="en">accessPTS</rdfs:label>
    </owl:ObjectProperty>
    


    <!-- https://w3id.org/transmodel/journeys#allowedLineDirections -->

    <owl:ObjectProperty rdf:about="https://w3id.org/transmodel/journeys#allowedLineDirections">
        <rdfs:subPropertyOf rdf:resource="https://w3id.org/transmodel/journeys#PROPS-TO-REVIEW"/>
        <rdfs:domain rdf:resource="https://w3id.org/transmodel/journeys#Route"/>
        <rdfs:range rdf:resource="https://w3id.org/transmodel/journeys#AllowedLineDirections"/>
        <rdfs:label xml:lang="en">allowedLineDirections</rdfs:label>
    </owl:ObjectProperty>
    


    <!-- https://w3id.org/transmodel/journeys#beginsConnection -->

    <owl:ObjectProperty rdf:about="https://w3id.org/transmodel/journeys#beginsConnection">
        <rdfs:subPropertyOf rdf:resource="https://w3id.org/transmodel/journeys#PROPS-TO-REVIEW"/>
        <rdfs:domain rdf:resource="https://w3id.org/transmodel/journeys#Connection"/>
        <rdfs:range rdf:resource="https://w3id.org/transmodel/journeys#ScheduledStopPoint"/>
        <rdfs:label xml:lang="en">beginsConnection</rdfs:label>
    </owl:ObjectProperty>
    


    <!-- https://w3id.org/transmodel/journeys#belongingTo -->

    <owl:ObjectProperty rdf:about="https://w3id.org/transmodel/journeys#belongingTo">
        <rdfs:domain rdf:resource="https://w3id.org/transmodel/facilities#VehicleType"/>
        <rdfs:range rdf:resource="https://w3id.org/transmodel/journeys#VehicleMode"/>
        <rdfs:comment xml:lang="en">This property sets the relationship between Vehicle Type and Vehicle Mode</rdfs:comment>
        <rdfs:label xml:lang="en">belonging To</rdfs:label>
    </owl:ObjectProperty>
    


    <!-- https://w3id.org/transmodel/journeys#blockPart -->

    <owl:ObjectProperty rdf:about="https://w3id.org/transmodel/journeys#blockPart">
        <rdfs:subPropertyOf rdf:resource="https://w3id.org/transmodel/journeys#PROPS-TO-REVIEW"/>
        <rdfs:domain rdf:resource="https://w3id.org/transmodel/journeys#JourneyPart"/>
        <rdfs:range rdf:resource="https://w3id.org/transmodel/journeys#BlockPart"/>
        <rdfs:label xml:lang="en">blockPart</rdfs:label>
    </owl:ObjectProperty>
    


    <!-- https://w3id.org/transmodel/journeys#canAlight -->

    <owl:ObjectProperty rdf:about="https://w3id.org/transmodel/journeys#canAlight">
        <rdfs:subPropertyOf rdf:resource="https://w3id.org/transmodel/journeys#PROPS-TO-REVIEW"/>
        <rdfs:range rdf:resource="https://w3id.org/transmodel/journeys#ScheduledStopPoint"/>
        <rdfs:label xml:lang="en">canAlight</rdfs:label>
    </owl:ObjectProperty>
    


    <!-- https://w3id.org/transmodel/journeys#canBoard -->

    <owl:ObjectProperty rdf:about="https://w3id.org/transmodel/journeys#canBoard">
        <rdfs:subPropertyOf rdf:resource="https://w3id.org/transmodel/journeys#PROPS-TO-REVIEW"/>
        <rdfs:range rdf:resource="https://w3id.org/transmodel/journeys#ScheduledStopPoint"/>
        <rdfs:label xml:lang="en">canBoard</rdfs:label>
    </owl:ObjectProperty>
    


    <!-- https://w3id.org/transmodel/journeys#characterisedBy -->

    <owl:ObjectProperty rdf:about="https://w3id.org/transmodel/journeys#characterisedBy">
        <rdfs:domain rdf:resource="https://w3id.org/transmodel/journeys#Journey"/>
        <rdfs:range rdf:resource="https://w3id.org/transmodel/facilities#AccessibilityAssessment"/>
        <rdfs:comment xml:lang="en">This property is the relationship of a Journey and the Accessibility Assessment</rdfs:comment>
        <rdfs:label xml:lang="en">characterised By</rdfs:label>
    </owl:ObjectProperty>
    


    <!-- https://w3id.org/transmodel/journeys#classifiedBy -->

    <owl:ObjectProperty rdf:about="https://w3id.org/transmodel/journeys#classifiedBy">
        <rdfs:domain rdf:resource="https://w3id.org/transmodel/journeys#Line"/>
        <rdfs:range>
            <owl:Class>
                <owl:intersectionOf rdf:parseType="Collection">
                    <rdf:Description rdf:about="http://www.w3.org/2004/02/skos/core#Concept"/>
                    <owl:Restriction>
                        <owl:onProperty rdf:resource="http://www.w3.org/2004/02/skos/core#inScheme"/>
                        <owl:hasValue rdf:resource="https://w3id.org/transmodel/kos/commons/all-modes"/>
                    </owl:Restriction>
                </owl:intersectionOf>
            </owl:Class>
        </rdfs:range>
        <rdfs:comment xml:lang="en">This property allows relating a Line with the transport modes which are used to operate it</rdfs:comment>
        <rdfs:label xml:lang="en">classified by</rdfs:label>
    </owl:ObjectProperty>
    


    <!-- https://w3id.org/transmodel/journeys#composedOf -->

    <owl:ObjectProperty rdf:about="https://w3id.org/transmodel/journeys#composedOf">
        <owl:inverseOf rdf:resource="https://w3id.org/transmodel/journeys#runsOn"/>
        <rdfs:domain rdf:resource="https://w3id.org/transmodel/journeys#VehicleJourney"/>
        <rdfs:range rdf:resource="https://w3id.org/transmodel/journeys#JourneyFrequencyGroup"/>
        <rdfs:comment xml:lang="en">This property relates a Journey Frequency Group with the Vehicle Journeys that it is composed of</rdfs:comment>
        <rdfs:label xml:lang="en">composed of</rdfs:label>
    </owl:ObjectProperty>
    


    <!-- https://w3id.org/transmodel/journeys#day -->

    <owl:ObjectProperty rdf:about="https://w3id.org/transmodel/journeys#day">
        <rdfs:range>
            <owl:Class>
                <owl:intersectionOf rdf:parseType="Collection">
                    <rdf:Description rdf:about="http://www.w3.org/2004/02/skos/core#Concept"/>
                    <owl:Restriction>
                        <owl:onProperty rdf:resource="http://www.w3.org/2004/02/skos/core#inScheme"/>
                        <owl:hasValue rdf:resource="https://w3id.org/transmodel/kos/journeys/day-type"/>
                    </owl:Restriction>
                </owl:intersectionOf>
            </owl:Class>
        </rdfs:range>
        <rdfs:comment xml:lang="en">This property relates a Day Of Week with a Day Type which is defined in KOS day-type</rdfs:comment>
        <rdfs:label xml:lang="en">day</rdfs:label>
    </owl:ObjectProperty>
    


    <!-- https://w3id.org/transmodel/journeys#dayTypeAssignment -->

    <owl:ObjectProperty rdf:about="https://w3id.org/transmodel/journeys#dayTypeAssignment">
        <rdfs:subPropertyOf rdf:resource="https://w3id.org/transmodel/journeys#PROPS-TO-REVIEW"/>
        <rdfs:comment xml:lang="en">The assignment of operational characteristics, expressed by DayType, to a particular OperatingDay within a ServiceCalendar</rdfs:comment>
        <rdfs:label xml:lang="en">dayTypeAssignment</rdfs:label>
    </owl:ObjectProperty>
    


    <!-- https://w3id.org/transmodel/journeys#defaultDeadRunRunTime -->

    <owl:ObjectProperty rdf:about="https://w3id.org/transmodel/journeys#defaultDeadRunRunTime">
        <rdfs:subPropertyOf rdf:resource="https://w3id.org/transmodel/journeys#PROPS-TO-REVIEW"/>
        <rdfs:domain rdf:resource="https://w3id.org/transmodel/journeys#DeadRun"/>
        <rdfs:range rdf:resource="https://w3id.org/transmodel/journeys#TimingLink"/>
        <rdfs:label xml:lang="en">defaultDeadRunRunTime</rdfs:label>
    </owl:ObjectProperty>
    


    <!-- https://w3id.org/transmodel/journeys#defaultInterchange -->

    <owl:ObjectProperty rdf:about="https://w3id.org/transmodel/journeys#defaultInterchange">
        <rdfs:subPropertyOf rdf:resource="https://w3id.org/transmodel/journeys#PROPS-TO-REVIEW"/>
        <rdfs:domain rdf:resource="https://w3id.org/transmodel/journeys#ScheduledStopPoint"/>
        <rdfs:range rdf:resource="https://w3id.org/transmodel/journeys#DefaultInterchange"/>
        <rdfs:label xml:lang="en">defaultInterchange</rdfs:label>
    </owl:ObjectProperty>
    


    <!-- https://w3id.org/transmodel/journeys#definedAs -->

    <owl:ObjectProperty rdf:about="https://w3id.org/transmodel/journeys#definedAs">
        <rdfs:domain rdf:resource="https://w3id.org/transmodel/journeys#PropertyOfDay"/>
        <rdfs:range>
            <owl:Class>
                <owl:intersectionOf rdf:parseType="Collection">
                    <rdf:Description rdf:about="http://www.w3.org/2004/02/skos/core#Concept"/>
                    <owl:Restriction>
                        <owl:onProperty rdf:resource="http://www.w3.org/2004/02/skos/core#inScheme"/>
                        <owl:hasValue rdf:resource="https://w3id.org/transmodel/kos/journeys/day-type"/>
                    </owl:Restriction>
                </owl:intersectionOf>
            </owl:Class>
        </rdfs:range>
        <rdfs:comment xml:lang="en">This property sets the relationship between Property Of Day and the SKOS Concept Scheme for days of the week</rdfs:comment>
        <rdfs:label xml:lang="en">defined As</rdfs:label>
    </owl:ObjectProperty>
    


    <!-- https://w3id.org/transmodel/journeys#defines -->

    <owl:ObjectProperty rdf:about="https://w3id.org/transmodel/journeys#defines">
        <owl:inverseOf rdf:resource="https://w3id.org/transmodel/journeys#isDefinedBy"/>
        <rdfs:domain rdf:resource="https://w3id.org/transmodel/journeys#RhythmicalJourneyGroup"/>
        <rdfs:range rdf:resource="https://w3id.org/transmodel/journeys#TemplateVehicleJourney"/>
        <rdfs:comment xml:lang="en">This property relates a Rhythmical Journey Group with a Template Vehicle Journey</rdfs:comment>
        <rdfs:label xml:lang="en">defines</rdfs:label>
    </owl:ObjectProperty>
    


    <!-- https://w3id.org/transmodel/journeys#describedBy -->

    <owl:ObjectProperty rdf:about="https://w3id.org/transmodel/journeys#describedBy">
        <rdfs:subPropertyOf rdf:resource="http://www.w3.org/2002/07/owl#topObjectProperty"/>
        <rdfs:domain rdf:resource="https://w3id.org/transmodel/journeys#DayType"/>
        <rdfs:range rdf:resource="https://w3id.org/transmodel/journeys#PropertyOfDay"/>
        <rdfs:comment xml:lang="en">This property asign a DayType to the specific Property of Day</rdfs:comment>
        <rdfs:label xml:lang="en">described By</rdfs:label>
    </owl:ObjectProperty>
    


    <!-- https://w3id.org/transmodel/journeys#destinationDisplay -->

    <owl:ObjectProperty rdf:about="https://w3id.org/transmodel/journeys#destinationDisplay">
        <rdfs:range rdf:resource="https://w3id.org/transmodel/journeys#DestinationDisplay"/>
        <rdfs:label xml:lang="en">destination display</rdfs:label>
    </owl:ObjectProperty>
    


    <!-- https://w3id.org/transmodel/journeys#destinationStop -->

    <owl:ObjectProperty rdf:about="https://w3id.org/transmodel/journeys#destinationStop">
        <rdfs:subPropertyOf rdf:resource="https://w3id.org/transmodel/journeys#PROPS-TO-REVIEW"/>
        <rdfs:range rdf:resource="https://w3id.org/transmodel/journeys#ScheduledStopPoint"/>
        <rdfs:label xml:lang="en">destinationStop</rdfs:label>
    </owl:ObjectProperty>
    


    <!-- https://w3id.org/transmodel/journeys#determinedBy -->

    <owl:ObjectProperty rdf:about="https://w3id.org/transmodel/journeys#determinedBy">
        <rdfs:domain rdf:resource="https://w3id.org/transmodel/journeys#HeadwayJourneyGroup"/>
        <rdfs:range rdf:resource="https://w3id.org/transmodel/journeys#HeadwayInterval"/>
    </owl:ObjectProperty>
    


    <!-- https://w3id.org/transmodel/journeys#directionType -->

    <owl:ObjectProperty rdf:about="https://w3id.org/transmodel/journeys#directionType">
        <rdfs:subPropertyOf rdf:resource="http://www.w3.org/2002/07/owl#topObjectProperty"/>
        <rdfs:domain rdf:resource="https://w3id.org/transmodel/journeys#ServiceJourney"/>
        <rdfs:range>
            <owl:Class>
                <owl:intersectionOf rdf:parseType="Collection">
                    <rdf:Description rdf:about="http://www.w3.org/2004/02/skos/core#Concept"/>
                    <owl:Restriction>
                        <owl:onProperty rdf:resource="http://www.w3.org/2004/02/skos/core#inScheme"/>
                        <owl:hasValue rdf:resource="https://w3id.org/transmodel/kos/journeys/direction-type"/>
                    </owl:Restriction>
                </owl:intersectionOf>
            </owl:Class>
        </rdfs:range>
        <rdfs:comment xml:lang="en">This property allows describing the type of direction for a service journey</rdfs:comment>
        <rdfs:label xml:lang="en">direction Type</rdfs:label>
    </owl:ObjectProperty>
    


    <!-- https://w3id.org/transmodel/journeys#directionType_old -->

    <owl:ObjectProperty rdf:about="https://w3id.org/transmodel/journeys#directionType_old">
        <rdfs:subPropertyOf rdf:resource="https://w3id.org/transmodel/journeys#PROPS-TO-REVIEW"/>
        <rdfs:label xml:lang="en">direction Type</rdfs:label>
    </owl:ObjectProperty>
    


    <!-- https://w3id.org/transmodel/journeys#endOfBlock -->

    <owl:ObjectProperty rdf:about="https://w3id.org/transmodel/journeys#endOfBlock">
        <rdfs:domain rdf:resource="https://w3id.org/transmodel/journeys#ParkingPoint"/>
        <rdfs:range rdf:resource="https://w3id.org/transmodel/journeys#Block"/>
        <rdfs:comment xml:lang="en">Property to relate a Parking Point to the end of a Block</rdfs:comment>
        <rdfs:label xml:lang="en">end of block</rdfs:label>
    </owl:ObjectProperty>
    


    <!-- https://w3id.org/transmodel/journeys#endingAt -->

    <owl:ObjectProperty rdf:about="https://w3id.org/transmodel/journeys#endingAt">
        <rdfs:domain rdf:resource="https://w3id.org/transmodel/journeys#OperatingPeriod"/>
        <rdfs:range rdf:resource="https://w3id.org/transmodel/journeys#OperatingDay"/>
        <rdfs:comment xml:lang="en">Property to connect an Operating Period to the related Operating Days, indicating when it ends</rdfs:comment>
        <rdfs:label xml:lang="en">ending at</rdfs:label>
    </owl:ObjectProperty>
    


    <!-- https://w3id.org/transmodel/journeys#endsConnection -->

    <owl:ObjectProperty rdf:about="https://w3id.org/transmodel/journeys#endsConnection">
        <rdfs:subPropertyOf rdf:resource="https://w3id.org/transmodel/journeys#PROPS-TO-REVIEW"/>
        <rdfs:domain rdf:resource="https://w3id.org/transmodel/journeys#Connection"/>
        <rdfs:range rdf:resource="https://w3id.org/transmodel/journeys#ScheduledStopPoint"/>
        <rdfs:comment xml:lang="en">Connection End, one end of a connection in Transmodel v6.0</rdfs:comment>
        <rdfs:label xml:lang="en">endsConnection</rdfs:label>
    </owl:ObjectProperty>
    


    <!-- https://w3id.org/transmodel/journeys#endsConnectionDefault -->

    <owl:ObjectProperty rdf:about="https://w3id.org/transmodel/journeys#endsConnectionDefault">
        <rdfs:subPropertyOf rdf:resource="https://w3id.org/transmodel/journeys#endsConnection"/>
        <rdfs:domain rdf:resource="https://w3id.org/transmodel/journeys#DefaultConnection"/>
        <rdfs:range rdf:resource="https://w3id.org/transmodel/journeys#ScheduledStopPoint"/>
        <rdfs:label xml:lang="en">endsConnectionDefault</rdfs:label>
    </owl:ObjectProperty>
    


    <!-- https://w3id.org/transmodel/journeys#followsDeadRunTime -->

    <owl:ObjectProperty rdf:about="https://w3id.org/transmodel/journeys#followsDeadRunTime">
        <rdfs:subPropertyOf rdf:resource="https://w3id.org/transmodel/journeys#PROPS-TO-REVIEW"/>
        <rdfs:domain rdf:resource="https://w3id.org/transmodel/journeys#VehicleJourney"/>
        <rdfs:range rdf:resource="https://w3id.org/transmodel/journeys#DeadRunPattern"/>
        <rdfs:label xml:lang="en">followsDeadRunPattern</rdfs:label>
    </owl:ObjectProperty>
    


    <!-- https://w3id.org/transmodel/journeys#followsJourneyPattern -->

    <owl:ObjectProperty rdf:about="https://w3id.org/transmodel/journeys#followsJourneyPattern">
        <rdfs:subPropertyOf rdf:resource="https://w3id.org/transmodel/journeys#PROPS-TO-REVIEW"/>
        <rdfs:domain rdf:resource="https://w3id.org/transmodel/journeys#VehicleJourney"/>
        <rdfs:range rdf:resource="https://w3id.org/transmodel/journeys#JourneyPattern"/>
        <rdfs:label xml:lang="en">followsJourneyPattern</rdfs:label>
    </owl:ObjectProperty>
    


    <!-- https://w3id.org/transmodel/journeys#for -->

    <owl:ObjectProperty rdf:about="https://w3id.org/transmodel/journeys#for">
        <rdfs:domain rdf:resource="https://w3id.org/transmodel/journeys#StopAssignment"/>
        <rdfs:comment xml:lang="en">A general property that allows associating a Stop Assignment to a Scheduled Stop Point, Quay, Boarding Position and/or Stop Place</rdfs:comment>
        <rdfs:label xml:lang="en">for</rdfs:label>
    </owl:ObjectProperty>
    


    <!-- https://w3id.org/transmodel/journeys#forServicedOrganisation -->

    <owl:ObjectProperty rdf:about="https://w3id.org/transmodel/journeys#forServicedOrganisation">
        <rdfs:domain rdf:resource="https://w3id.org/transmodel/journeys#OrganisationDayType"/>
        <rdfs:comment xml:lang="en">TODO: Add range tmorg:ServicedOrganisation</rdfs:comment>
        <rdfs:comment xml:lang="en">This property connects an Organisation Day Type to a Service Organisation, indicating that such Day Type is for providing service to the corresponding Organisation</rdfs:comment>
        <rdfs:label xml:lang="en">for serviced organisation</rdfs:label>
    </owl:ObjectProperty>
    


    <!-- https://w3id.org/transmodel/journeys#holidayType -->

    <owl:ObjectProperty rdf:about="https://w3id.org/transmodel/journeys#holidayType">
        <rdfs:range>
            <owl:Class>
                <owl:intersectionOf rdf:parseType="Collection">
                    <rdf:Description rdf:about="http://www.w3.org/2004/02/skos/core#Concept"/>
                    <owl:Restriction>
                        <owl:onProperty rdf:resource="http://www.w3.org/2004/02/skos/core#inScheme"/>
                        <owl:hasValue rdf:resource="https://w3id.org/transmodel/kos/journeys/day-type"/>
                    </owl:Restriction>
                </owl:intersectionOf>
            </owl:Class>
        </rdfs:range>
        <rdfs:comment xml:lang="en">This propery sets the relationship with holiday type defined in the KOS day-type</rdfs:comment>
        <rdfs:label xml:lang="en">holiday Type</rdfs:label>
    </owl:ObjectProperty>
    


    <!-- https://w3id.org/transmodel/journeys#inLinkSequence -->

    <owl:ObjectProperty rdf:about="https://w3id.org/transmodel/journeys#inLinkSequence">
        <rdfs:subPropertyOf rdf:resource="http://www.w3.org/2002/07/owl#topObjectProperty"/>
        <owl:inverseOf rdf:resource="https://w3id.org/transmodel/journeys#madeUpOf"/>
        <rdf:type rdf:resource="http://www.w3.org/2002/07/owl#FunctionalProperty"/>
        <rdfs:domain rdf:resource="https://w3id.org/transmodel/journeys#PointInLinkSequence"/>
        <rdfs:range rdf:resource="https://w3id.org/transmodel/journeys#LinkSequence"/>
        <rdfs:comment xml:lang="en">This property allows relating a Point in Link Sequence with the corresponding Link Sequence</rdfs:comment>
        <rdfs:label xml:lang="en">in Link Sequence</rdfs:label>
    </owl:ObjectProperty>
    


    <!-- https://w3id.org/transmodel/journeys#isDefinedBy -->

    <owl:ObjectProperty rdf:about="https://w3id.org/transmodel/journeys#isDefinedBy">
        <rdfs:domain rdf:resource="https://w3id.org/transmodel/journeys#TemplateVehicleJourney"/>
        <rdfs:range rdf:resource="https://w3id.org/transmodel/journeys#RhythmicalJourneyGroup"/>
        <rdfs:comment xml:lang="en">This property relates a Template Vehicle Journey with the Rhythmical Journey Group that defines it</rdfs:comment>
        <rdfs:label xml:lang="en">is defined by</rdfs:label>
    </owl:ObjectProperty>
    


    <!-- https://w3id.org/transmodel/journeys#journeyPatternMadeUpOf -->

    <owl:ObjectProperty rdf:about="https://w3id.org/transmodel/journeys#journeyPatternMadeUpOf">
        <rdfs:subPropertyOf rdf:resource="https://w3id.org/transmodel/journeys#PROPS-TO-REVIEW"/>
        <rdfs:domain rdf:resource="https://w3id.org/transmodel/facilities#JourneyPattern"/>
        <rdfs:range rdf:resource="https://w3id.org/transmodel/journeys#StopPointInJourneyPattern"/>
        <rdfs:comment xml:lang="en">A Journey Pattern is Made Up Of Stop Point In Journey Pattern</rdfs:comment>
        <rdfs:comment xml:lang="en">TODO: change to madeUpOf</rdfs:comment>
        <rdfs:label xml:lang="en">journey Pattern Made Up Of</rdfs:label>
    </owl:ObjectProperty>
    


    <!-- https://w3id.org/transmodel/journeys#journeyPatternPoint -->

    <owl:ObjectProperty rdf:about="https://w3id.org/transmodel/journeys#journeyPatternPoint">
        <rdfs:subPropertyOf rdf:resource="https://w3id.org/transmodel/journeys#PROPS-TO-REVIEW"/>
        <rdfs:domain rdf:resource="https://w3id.org/transmodel/journeys#JourneyPattern"/>
        <rdfs:range rdf:resource="https://w3id.org/transmodel/journeys#Point"/>
        <rdfs:label xml:lang="en">journeyPatternPoint</rdfs:label>
    </owl:ObjectProperty>
    


    <!-- https://w3id.org/transmodel/journeys#journeyPatternRunTime -->

    <owl:ObjectProperty rdf:about="https://w3id.org/transmodel/journeys#journeyPatternRunTime">
        <rdfs:subPropertyOf rdf:resource="https://w3id.org/transmodel/journeys#PROPS-TO-REVIEW"/>
        <rdfs:domain rdf:resource="https://w3id.org/transmodel/journeys#JourneyPattern"/>
        <rdfs:range rdf:resource="https://w3id.org/transmodel/journeys#TimingLink"/>
        <rdfs:label xml:lang="en">journeyRunTime</rdfs:label>
    </owl:ObjectProperty>
    


    <!-- https://w3id.org/transmodel/journeys#madeUpOf -->

    <owl:ObjectProperty rdf:about="https://w3id.org/transmodel/journeys#madeUpOf">
        <rdfs:subPropertyOf rdf:resource="http://www.w3.org/2002/07/owl#topObjectProperty"/>
        <rdfs:domain rdf:resource="https://w3id.org/transmodel/journeys#LinkSequence"/>
        <rdfs:range rdf:resource="https://w3id.org/transmodel/journeys#PointInLinkSequence"/>
        <rdfs:comment xml:lang="en">This property allows relating a Link Sequence with the set of Points in Link Sequence that make it up</rdfs:comment>
        <rdfs:label xml:lang="en">made Up Of</rdfs:label>
    </owl:ObjectProperty>
    


    <!-- https://w3id.org/transmodel/journeys#madeUsing -->

    <owl:ObjectProperty rdf:about="https://w3id.org/transmodel/journeys#madeUsing">
        <rdfs:subPropertyOf rdf:resource="http://www.w3.org/2002/07/owl#topObjectProperty"/>
        <rdfs:domain rdf:resource="https://w3id.org/transmodel/journeys#ServiceJourney"/>
        <rdfs:range rdf:resource="https://w3id.org/transmodel/facilities#ServiceFacilitySet"/>
        <rdfs:comment xml:lang="en">This property connects a Service Journey to the Service Facility Set that is making it possible</rdfs:comment>
        <rdfs:label xml:lang="en">made Using</rdfs:label>
    </owl:ObjectProperty>
    


    <!-- https://w3id.org/transmodel/journeys#modeOfTransport -->

    <owl:ObjectProperty rdf:about="https://w3id.org/transmodel/journeys#modeOfTransport">
        <rdfs:subPropertyOf rdf:resource="https://w3id.org/transmodel/journeys#PROPS-TO-REVIEW"/>
        <rdfs:domain rdf:resource="https://w3id.org/transmodel/journeys#Route"/>
        <rdfs:range rdf:resource="https://w3id.org/transmodel/journeys#MeanOfTransport"/>
    </owl:ObjectProperty>
    


    <!-- https://w3id.org/transmodel/journeys#on -->

    <owl:ObjectProperty rdf:about="https://w3id.org/transmodel/journeys#on">
        <rdfs:subPropertyOf rdf:resource="http://www.w3.org/2002/07/owl#topObjectProperty"/>
        <rdfs:comment xml:lang="en">This property allows relating an entity with the entity where it appears. For instance, a Journey Pattern on (onRoute) a Route, a Route on (onLine) a Line.</rdfs:comment>
        <rdfs:label xml:lang="en">on</rdfs:label>
    </owl:ObjectProperty>
    


    <!-- https://w3id.org/transmodel/journeys#onLine -->

    <owl:ObjectProperty rdf:about="https://w3id.org/transmodel/journeys#onLine">
        <rdfs:subPropertyOf rdf:resource="https://w3id.org/transmodel/journeys#on"/>
        <rdfs:domain rdf:resource="https://w3id.org/transmodel/journeys#Line"/>
        <rdfs:range rdf:resource="https://w3id.org/transmodel/journeys#Route"/>
        <rdfs:comment xml:lang="en">This property allows relating a Route with a Line where it appears</rdfs:comment>
        <rdfs:label xml:lang="en">on Line</rdfs:label>
    </owl:ObjectProperty>
    


    <!-- https://w3id.org/transmodel/journeys#onRoute -->

    <owl:ObjectProperty rdf:about="https://w3id.org/transmodel/journeys#onRoute">
        <rdfs:subPropertyOf rdf:resource="https://w3id.org/transmodel/journeys#on"/>
        <rdfs:domain rdf:resource="https://w3id.org/transmodel/journeys#Route"/>
        <rdfs:range rdf:resource="https://w3id.org/transmodel/journeys#ServiceJourneyPattern"/>
        <rdfs:comment xml:lang="en">This property allows relating a Journey Pattern with a Route where it appears</rdfs:comment>
        <rdfs:label xml:lang="en">on Route</rdfs:label>
    </owl:ObjectProperty>
    


    <!-- https://w3id.org/transmodel/journeys#operatedBy -->

    <owl:ObjectProperty rdf:about="https://w3id.org/transmodel/journeys#operatedBy">
        <rdfs:domain rdf:resource="https://w3id.org/transmodel/journeys#VehicleJourney"/>
        <rdfs:range rdf:resource="https://w3id.org/transmodel/facilities#VehicleType"/>
        <rdfs:comment xml:lang="en">This property sets the relationship between a Vehicle Journey and a Vehicle Type</rdfs:comment>
        <rdfs:label xml:lang="en">operated By</rdfs:label>
    </owl:ObjectProperty>
    


    <!-- https://w3id.org/transmodel/journeys#operatingPeriod -->

    <owl:ObjectProperty rdf:about="https://w3id.org/transmodel/journeys#operatingPeriod">
        <rdfs:range rdf:resource="https://w3id.org/transmodel/journeys#OperatingPeriod"/>
        <rdfs:comment xml:lang="en">operating period</rdfs:comment>
        <rdfs:comment xml:lang="en">operating period assigned to a Day Type Assignment</rdfs:comment>
    </owl:ObjectProperty>
    


    <!-- https://w3id.org/transmodel/journeys#originStop -->

    <owl:ObjectProperty rdf:about="https://w3id.org/transmodel/journeys#originStop">
        <rdfs:subPropertyOf rdf:resource="https://w3id.org/transmodel/journeys#PROPS-TO-REVIEW"/>
        <rdfs:range rdf:resource="https://w3id.org/transmodel/journeys#ScheduledStopPoint"/>
        <rdfs:label xml:lang="en">originStop</rdfs:label>
    </owl:ObjectProperty>
    


    <!-- https://w3id.org/transmodel/journeys#overriding -->

    <owl:ObjectProperty rdf:about="https://w3id.org/transmodel/journeys#overriding">
        <rdfs:domain rdf:resource="https://w3id.org/transmodel/journeys#DynamicStopAssignment"/>
        <rdfs:range rdf:resource="https://w3id.org/transmodel/journeys#PassengerStopAssignment"/>
        <rdfs:comment xml:lang="en">This property is used to specify the Passenger Stop Assignment that a Dynamic Stop Assignment overrides</rdfs:comment>
        <rdfs:label xml:lang="en">overriding</rdfs:label>
    </owl:ObjectProperty>
    


    <!-- https://w3id.org/transmodel/journeys#passengerConnection -->

    <owl:ObjectProperty rdf:about="https://w3id.org/transmodel/journeys#passengerConnection">
        <rdfs:subPropertyOf rdf:resource="https://w3id.org/transmodel/journeys#PROPS-TO-REVIEW"/>
        <rdfs:range rdf:resource="https://w3id.org/transmodel/journeys#Connection"/>
        <rdfs:label xml:lang="en">passengerConnection</rdfs:label>
    </owl:ObjectProperty>
    


    <!-- https://w3id.org/transmodel/journeys#passesAt -->

    <owl:ObjectProperty rdf:about="https://w3id.org/transmodel/journeys#passesAt">
        <rdfs:comment xml:lang="en">TODO: Check which domain and range to use</rdfs:comment>
        <rdfs:comment xml:lang="en">This property sets the relationship between a Point In Journey Pattern or a Service Journey and a Timetabled Passing Time</rdfs:comment>
        <rdfs:label xml:lang="en">passes at</rdfs:label>
    </owl:ObjectProperty>
    


    <!-- https://w3id.org/transmodel/journeys#passingTimeTimingPoint -->

    <owl:ObjectProperty rdf:about="https://w3id.org/transmodel/journeys#passingTimeTimingPoint">
        <rdfs:subPropertyOf rdf:resource="https://w3id.org/transmodel/journeys#PROPS-TO-REVIEW"/>
        <rdfs:range rdf:resource="https://w3id.org/transmodel/journeys#TimingPoint"/>
        <rdfs:label>passingTimeTimingPoint</rdfs:label>
    </owl:ObjectProperty>
    


    <!-- https://w3id.org/transmodel/journeys#prescribing -->

    <owl:ObjectProperty rdf:about="https://w3id.org/transmodel/journeys#prescribing">
        <rdfs:subPropertyOf rdf:resource="http://www.w3.org/2002/07/owl#topObjectProperty"/>
        <rdfs:domain rdf:resource="https://w3id.org/transmodel/journeys#PointInJourneyPattern"/>
        <rdfs:range rdf:resource="https://w3id.org/transmodel/journeys#DestinationDisplay"/>
        <rdfs:comment xml:lang="en">This property relates a Point in Journey Pattern with a Destination Display</rdfs:comment>
        <rdfs:label xml:lang="en">prescribing</rdfs:label>
    </owl:ObjectProperty>
    


    <!-- https://w3id.org/transmodel/journeys#presentedBy -->

    <owl:ObjectProperty rdf:about="https://w3id.org/transmodel/journeys#presentedBy">
        <rdfs:domain rdf:resource="https://w3id.org/transmodel/journeys#Line"/>
        <rdfs:range rdf:resource="https://w3id.org/transmodel/commons#Presentation"/>
        <rdfs:comment xml:lang="en">This property is used to connect a Line with its corresponding Presentation</rdfs:comment>
        <rdfs:label xml:lang="en">presented by</rdfs:label>
    </owl:ObjectProperty>
    


    <!-- https://w3id.org/transmodel/journeys#primarilyAdvertisedWith -->

    <owl:ObjectProperty rdf:about="https://w3id.org/transmodel/journeys#primarilyAdvertisedWith">
        <rdfs:subPropertyOf rdf:resource="http://www.w3.org/2002/07/owl#topObjectProperty"/>
        <rdfs:domain rdf:resource="https://w3id.org/transmodel/journeys#JourneyPattern"/>
        <rdfs:range rdf:resource="https://w3id.org/transmodel/journeys#DestinationDisplay"/>
        <rdfs:comment xml:lang="en">This property relates where is primarily advertised the Journey Pattern in a Destination Display</rdfs:comment>
        <rdfs:label xml:lang="en">primarily Advertised With</rdfs:label>
    </owl:ObjectProperty>
    


    <!-- https://w3id.org/transmodel/journeys#routeOnLine -->

    <owl:ObjectProperty rdf:about="https://w3id.org/transmodel/journeys#routeOnLine">
        <rdfs:subPropertyOf rdf:resource="https://w3id.org/transmodel/journeys#PROPS-TO-REVIEW"/>
        <rdfs:domain rdf:resource="https://w3id.org/transmodel/journeys#Line-old"/>
        <rdfs:range rdf:resource="https://w3id.org/transmodel/journeys#Route"/>
        <rdfs:label xml:lang="en">route On Line</rdfs:label>
    </owl:ObjectProperty>
    


    <!-- https://w3id.org/transmodel/journeys#runBy -->

    <owl:ObjectProperty rdf:about="https://w3id.org/transmodel/journeys#runBy">
        <rdfs:subPropertyOf rdf:resource="http://www.w3.org/2002/07/owl#topObjectProperty"/>
        <rdfs:domain rdf:resource="https://w3id.org/transmodel/journeys#Line"/>
        <rdfs:range rdf:resource="https://w3id.org/transmodel/organisations#Operator"/>
        <rdfs:comment xml:lang="en">A Line is run by an Operator</rdfs:comment>
        <rdfs:label xml:lang="en">run By</rdfs:label>
    </owl:ObjectProperty>
    


    <!-- https://w3id.org/transmodel/journeys#runTimeOverrides -->

    <owl:ObjectProperty rdf:about="https://w3id.org/transmodel/journeys#runTimeOverrides">
        <rdfs:subPropertyOf rdf:resource="https://w3id.org/transmodel/journeys#PROPS-TO-REVIEW"/>
        <rdfs:range rdf:resource="https://w3id.org/transmodel/journeys#DefaultDeadRunRunTime"/>
        <rdfs:range rdf:resource="https://w3id.org/transmodel/journeys#DefaultServiceJourneyRunTime"/>
        <rdfs:label xml:lang="en">journeyRunTimeOverrides</rdfs:label>
    </owl:ObjectProperty>
    


    <!-- https://w3id.org/transmodel/journeys#runsOn -->

    <owl:ObjectProperty rdf:about="https://w3id.org/transmodel/journeys#runsOn">
        <rdfs:domain rdf:resource="https://w3id.org/transmodel/journeys#JourneyFrequencyGroup"/>
        <rdfs:range rdf:resource="https://w3id.org/transmodel/journeys#VehicleJourney"/>
        <rdfs:comment xml:lang="en">This property relates a Vehicle Journey with the Journey Frequency Group(s) that it belongs to</rdfs:comment>
        <rdfs:label xml:lang="en">runs On</rdfs:label>
    </owl:ObjectProperty>
    


    <!-- https://w3id.org/transmodel/journeys#scheduledStopPoint -->

    <owl:ObjectProperty rdf:about="https://w3id.org/transmodel/journeys#scheduledStopPoint">
        <rdfs:subPropertyOf rdf:resource="https://w3id.org/transmodel/journeys#PROPS-TO-REVIEW"/>
        <rdfs:domain rdf:resource="https://w3id.org/transmodel/journeys#Route"/>
        <rdfs:range rdf:resource="https://w3id.org/transmodel/journeys#ScheduledStopPoint"/>
        <rdfs:label xml:lang="en">scheduledStopPoint</rdfs:label>
    </owl:ObjectProperty>
    


    <!-- https://w3id.org/transmodel/journeys#season -->

    <owl:ObjectProperty rdf:about="https://w3id.org/transmodel/journeys#season">
        <rdfs:range>
            <owl:Class>
                <owl:intersectionOf rdf:parseType="Collection">
                    <rdf:Description rdf:about="http://www.w3.org/2004/02/skos/core#Concept"/>
                    <owl:Restriction>
                        <owl:onProperty rdf:resource="http://www.w3.org/2004/02/skos/core#inScheme"/>
                        <owl:hasValue rdf:resource="https://w3id.org/transmodel/kos/journeys/day-type"/>
                    </owl:Restriction>
                </owl:intersectionOf>
            </owl:Class>
        </rdfs:range>
        <rdfs:comment xml:lang="en">TODO: In journeys/daytype-properties there is the skos:Concept top concept season-type which must be the range of this property</rdfs:comment>
        <rdfs:comment xml:lang="en">This property states the season of a Operating Period</rdfs:comment>
        <rdfs:label xml:lang="en">season</rdfs:label>
    </owl:ObjectProperty>
    


    <!-- https://w3id.org/transmodel/journeys#serviceJourneyUsingPattern -->

    <owl:ObjectProperty rdf:about="https://w3id.org/transmodel/journeys#serviceJourneyUsingPattern">
        <rdfs:subPropertyOf rdf:resource="https://w3id.org/transmodel/journeys#PROPS-TO-REVIEW"/>
        <rdfs:domain rdf:resource="https://w3id.org/transmodel/journeys#ServiceJourney"/>
        <rdfs:range rdf:resource="https://w3id.org/transmodel/journeys#ServiceJourneyPattern"/>
        <rdfs:comment xml:lang="en">A Service Journey has (service Journey Pattern) a Service Journey Pattern</rdfs:comment>
        <rdfs:label xml:lang="en">service Journey Pattern</rdfs:label>
    </owl:ObjectProperty>
    


    <!-- https://w3id.org/transmodel/journeys#specifying -->

    <owl:ObjectProperty rdf:about="https://w3id.org/transmodel/journeys#specifying">
        <rdfs:subPropertyOf rdf:resource="http://www.w3.org/2002/07/owl#topObjectProperty"/>
        <rdfs:domain rdf:resource="https://w3id.org/transmodel/journeys#DayTypeAssignment"/>
        <rdfs:range rdf:resource="https://w3id.org/transmodel/journeys#DayType"/>
        <rdfs:comment xml:lang="en">The assignment of operational characteristics, expressed by DayType, to a particular OperatingDay within a ServiceCalendar</rdfs:comment>
        <rdfs:label xml:lang="en">specifying</rdfs:label>
    </owl:ObjectProperty>
    


    <!-- https://w3id.org/transmodel/journeys#startOfBlock -->

    <owl:ObjectProperty rdf:about="https://w3id.org/transmodel/journeys#startOfBlock">
        <rdfs:domain rdf:resource="https://w3id.org/transmodel/journeys#ParkingPoint"/>
        <rdfs:range rdf:resource="https://w3id.org/transmodel/journeys#Block"/>
        <rdfs:comment xml:lang="en">Property to relate a Parking Point to the start of a Block</rdfs:comment>
        <rdfs:label xml:lang="en">start Of Block</rdfs:label>
    </owl:ObjectProperty>
    


    <!-- https://w3id.org/transmodel/journeys#startingAt -->

    <owl:ObjectProperty rdf:about="https://w3id.org/transmodel/journeys#startingAt">
        <rdfs:domain rdf:resource="https://w3id.org/transmodel/journeys#OperatingPeriod"/>
        <rdfs:range rdf:resource="https://w3id.org/transmodel/journeys#OperatingDay"/>
        <rdfs:comment xml:lang="en">Property to connect an Operating Period to the related Operating Days, indicating when it starts</rdfs:comment>
        <rdfs:label xml:lang="en">starting At</rdfs:label>
    </owl:ObjectProperty>
    


    <!-- https://w3id.org/transmodel/journeys#stopUse -->

    <owl:ObjectProperty rdf:about="https://w3id.org/transmodel/journeys#stopUse">
        <rdfs:subPropertyOf rdf:resource="http://www.w3.org/2002/07/owl#topObjectProperty"/>
        <rdfs:domain rdf:resource="https://w3id.org/transmodel/journeys#StopPointInJourneyPattern"/>
        <rdfs:range>
            <owl:Class>
                <owl:intersectionOf rdf:parseType="Collection">
                    <rdf:Description rdf:about="http://www.w3.org/2004/02/skos/core#Concept"/>
                    <owl:Restriction>
                        <owl:onProperty rdf:resource="http://www.w3.org/2004/02/skos/core#inScheme"/>
                        <owl:hasValue rdf:resource="https://w3id.org/transmodel/kos/journeys/stop-use-type"/>
                    </owl:Restriction>
                </owl:intersectionOf>
            </owl:Class>
        </rdfs:range>
        <rdfs:comment xml:lang="en">This property allows describing the type of use of a stop (e.g., access, interchange only, pass through)</rdfs:comment>
        <rdfs:label xml:lang="en">stop Use</rdfs:label>
    </owl:ObjectProperty>
    


    <!-- https://w3id.org/transmodel/journeys#stopsAt -->

    <owl:ObjectProperty rdf:about="https://w3id.org/transmodel/journeys#stopsAt">
        <rdfs:subPropertyOf rdf:resource="https://w3id.org/transmodel/journeys#PROPS-TO-REVIEW"/>
        <rdfs:domain rdf:resource="https://w3id.org/transmodel/journeys#Vehicle"/>
        <rdfs:range rdf:resource="https://w3id.org/transmodel/journeys#ScheduledStopPoint"/>
        <rdfs:label xml:lang="en">stopsAt</rdfs:label>
    </owl:ObjectProperty>
    


    <!-- https://w3id.org/transmodel/journeys#timingLink -->

    <owl:ObjectProperty rdf:about="https://w3id.org/transmodel/journeys#timingLink">
        <rdfs:subPropertyOf rdf:resource="https://w3id.org/transmodel/journeys#PROPS-TO-REVIEW"/>
        <rdfs:domain rdf:resource="https://w3id.org/transmodel/journeys#TimingLink"/>
        <rdfs:range rdf:resource="https://w3id.org/transmodel/journeys#TimingPoint"/>
        <rdfs:label xml:lang="en">timingLinkPoint</rdfs:label>
    </owl:ObjectProperty>
    


    <!-- https://w3id.org/transmodel/journeys#timingLinkInJourneyPattern -->

    <owl:ObjectProperty rdf:about="https://w3id.org/transmodel/journeys#timingLinkInJourneyPattern">
        <rdfs:subPropertyOf rdf:resource="https://w3id.org/transmodel/journeys#PROPS-TO-REVIEW"/>
        <rdfs:domain rdf:resource="https://w3id.org/transmodel/journeys#JourneyPattern"/>
        <rdfs:range rdf:resource="https://w3id.org/transmodel/journeys#TimingLinkInJourneyPattern"/>
    </owl:ObjectProperty>
    


    <!-- https://w3id.org/transmodel/journeys#typeOfFlexibleService -->

    <owl:ObjectProperty rdf:about="https://w3id.org/transmodel/journeys#typeOfFlexibleService">
        <rdfs:subPropertyOf rdf:resource="https://w3id.org/transmodel/journeys#PROPS-TO-REVIEW"/>
        <rdfs:domain rdf:resource="https://w3id.org/transmodel/journeys#FlexibleLine"/>
        <rdfs:label>typeOfFlexibleService</rdfs:label>
    </owl:ObjectProperty>
    


    <!-- https://w3id.org/transmodel/journeys#usedToDefine -->

    <owl:ObjectProperty rdf:about="https://w3id.org/transmodel/journeys#usedToDefine">
        <rdfs:subPropertyOf rdf:resource="http://www.w3.org/2002/07/owl#topObjectProperty"/>
        <rdfs:domain rdf:resource="https://w3id.org/transmodel/journeys#OperatingDay"/>
        <rdfs:range rdf:resource="https://w3id.org/transmodel/journeys#DayTypeAssignment"/>
        <rdfs:comment xml:lang="en">This property sets the relation between a Time Band or an Operating Day with a Day Type Assignment</rdfs:comment>
        <rdfs:label xml:lang="en">used To Define</rdfs:label>
    </owl:ObjectProperty>
    


    <!-- https://w3id.org/transmodel/journeys#vehicleJourney -->

    <owl:ObjectProperty rdf:about="https://w3id.org/transmodel/journeys#vehicleJourney">
        <rdfs:subPropertyOf rdf:resource="https://w3id.org/transmodel/journeys#PROPS-TO-REVIEW"/>
        <rdfs:domain rdf:resource="https://w3id.org/transmodel/journeys#Vehicle"/>
        <rdfs:range rdf:resource="https://w3id.org/transmodel/journeys#VehicleJourney"/>
        <rdfs:comment xml:lang="en">A Vehicle makes (vehicleJourney) a Vehicle Journey</rdfs:comment>
        <rdfs:label xml:lang="en">vehicle Journey</rdfs:label>
    </owl:ObjectProperty>
    


    <!-- https://w3id.org/transmodel/journeys#vehicleJourneyPart -->

    <owl:ObjectProperty rdf:about="https://w3id.org/transmodel/journeys#vehicleJourneyPart">
        <rdfs:subPropertyOf rdf:resource="https://w3id.org/transmodel/journeys#PROPS-TO-REVIEW"/>
        <rdfs:domain rdf:resource="https://w3id.org/transmodel/journeys#Vehicle"/>
        <rdfs:range rdf:resource="https://w3id.org/transmodel/journeys#JourneyPart"/>
        <rdfs:label xml:lang="en">vehicleJourneyPart</rdfs:label>
    </owl:ObjectProperty>
    


    <!-- https://w3id.org/transmodel/journeys#vehicleJourneyRoute -->

    <owl:ObjectProperty rdf:about="https://w3id.org/transmodel/journeys#vehicleJourneyRoute">
        <rdfs:subPropertyOf rdf:resource="https://w3id.org/transmodel/journeys#PROPS-TO-REVIEW"/>
        <rdfs:domain rdf:resource="https://w3id.org/transmodel/journeys#VehicleJourney"/>
        <rdfs:range rdf:resource="https://w3id.org/transmodel/journeys#Route"/>
        <rdfs:label xml:lang="en">vehicleJourneyRoute</rdfs:label>
    </owl:ObjectProperty>
    


    <!-- https://w3id.org/transmodel/journeys#vehicleJourneyRunTimeOverrides -->

    <owl:ObjectProperty rdf:about="https://w3id.org/transmodel/journeys#vehicleJourneyRunTimeOverrides">
        <rdfs:subPropertyOf rdf:resource="https://w3id.org/transmodel/journeys#PROPS-TO-REVIEW"/>
        <rdfs:domain rdf:resource="https://w3id.org/transmodel/journeys#VehicleJourneyRunTime"/>
        <rdfs:range rdf:resource="https://w3id.org/transmodel/journeys#DefaultDeadRunRunTime"/>
        <rdfs:range rdf:resource="https://w3id.org/transmodel/journeys#DefaultServiceJourneyRunTime"/>
        <rdfs:range rdf:resource="https://w3id.org/transmodel/journeys#JourneyPatternRunTime"/>
        <rdfs:label xml:lang="en">vehicleJourneyRunTimeOverrides</rdfs:label>
    </owl:ObjectProperty>
    


    <!-- https://w3id.org/transmodel/journeys#vehicleJourneys -->

    <owl:ObjectProperty rdf:about="https://w3id.org/transmodel/journeys#vehicleJourneys">
        <rdfs:subPropertyOf rdf:resource="https://w3id.org/transmodel/journeys#PROPS-TO-REVIEW"/>
        <rdfs:domain rdf:resource="https://w3id.org/transmodel/journeys#Vehicle"/>
        <rdfs:range rdf:resource="https://w3id.org/transmodel/journeys#VehicleJourney"/>
        <rdfs:comment xml:lang="en">The Journey of a Vehicle is a VehicleJourney</rdfs:comment>
        <rdfs:label xml:lang="en">vehicleJourneys</rdfs:label>
    </owl:ObjectProperty>
    


    <!-- https://w3id.org/transmodel/journeys#vehicleModeId -->

    <owl:ObjectProperty rdf:about="https://w3id.org/transmodel/journeys#vehicleModeId">
        <rdfs:domain rdf:resource="https://w3id.org/transmodel/journeys#VehicleMode"/>
        <rdfs:range>
            <owl:Class>
                <owl:intersectionOf rdf:parseType="Collection">
                    <rdf:Description rdf:about="http://www.w3.org/2004/02/skos/core#Concept"/>
                    <owl:Restriction>
                        <owl:onProperty rdf:resource="http://www.w3.org/2004/02/skos/core#inScheme"/>
                        <owl:hasValue rdf:resource="https://w3id.org/transmodel/kos/journeys/day-type"/>
                    </owl:Restriction>
                </owl:intersectionOf>
            </owl:Class>
        </rdfs:range>
        <rdfs:comment xml:lang="en">This property sets the relationship between a Vehicle Mode and the type of Vehicle used defined in the kos/journeys/all-modes.ttl</rdfs:comment>
        <rdfs:label xml:lang="en">vehicle Mode ID</rdfs:label>
    </owl:ObjectProperty>
    


    <!-- https://w3id.org/transmodel/journeys#vehiclePassingTime -->

    <owl:ObjectProperty rdf:about="https://w3id.org/transmodel/journeys#vehiclePassingTime">
        <rdfs:subPropertyOf rdf:resource="https://w3id.org/transmodel/journeys#PROPS-TO-REVIEW"/>
        <rdfs:domain rdf:resource="https://w3id.org/transmodel/journeys#Vehicle"/>
        <rdfs:label xml:lang="en">vehiclePassingTime</rdfs:label>
    </owl:ObjectProperty>
    


    <!-- https://w3id.org/transmodel/journeys#viewedAs -->

    <owl:ObjectProperty rdf:about="https://w3id.org/transmodel/journeys#viewedAs">
        <rdfs:subPropertyOf rdf:resource="http://www.w3.org/2002/07/owl#topObjectProperty"/>
        <rdf:type rdf:resource="http://www.w3.org/2002/07/owl#FunctionalProperty"/>
        <rdfs:domain rdf:resource="https://w3id.org/transmodel/journeys#PointInLinkSequence"/>
        <rdfs:range rdf:resource="https://w3id.org/transmodel/journeys#Point"/>
        <rdfs:comment xml:lang="en">This property allows connecting a Point in Link Sequence with the corresponding Point</rdfs:comment>
        <rdfs:label xml:lang="en">viewed As</rdfs:label>
    </owl:ObjectProperty>
    


    <!-- https://w3id.org/transmodel/journeys#workedOn -->

    <owl:ObjectProperty rdf:about="https://w3id.org/transmodel/journeys#workedOn">
        <rdfs:domain rdf:resource="https://w3id.org/transmodel/journeys#VehicleJourney"/>
        <rdfs:range rdf:resource="https://w3id.org/transmodel/journeys#DayType"/>
        <rdfs:comment xml:lang="en">This property sets the relationship between Vehicle Journey and Day Type.</rdfs:comment>
        <rdfs:label xml:lang="en">worked On</rdfs:label>
    </owl:ObjectProperty>
    


    <!-- https://w3id.org/transmodel/organisations#passengerJourney -->

    <owl:ObjectProperty rdf:about="https://w3id.org/transmodel/organisations#passengerJourney">
        <rdfs:subPropertyOf rdf:resource="https://w3id.org/transmodel/journeys#PROPS-TO-REVIEW"/>
        <rdfs:range rdf:resource="https://w3id.org/transmodel/journeys#Trip"/>
        <rdfs:comment xml:lang="en">A Passenger makes (journey) a Trip</rdfs:comment>
        <rdfs:label xml:lang="en">passengerJourney</rdfs:label>
    </owl:ObjectProperty>
    


    <!-- https://w3id.org/transmodel/organisations#serviceJourneyServedByVehicleJourney -->

    <owl:ObjectProperty rdf:about="https://w3id.org/transmodel/organisations#serviceJourneyServedByVehicleJourney">
        <rdfs:subPropertyOf rdf:resource="https://w3id.org/transmodel/journeys#PROPS-TO-REVIEW"/>
        <rdfs:domain rdf:resource="https://w3id.org/transmodel/journeys#ServiceJourney"/>
        <rdfs:range rdf:resource="https://w3id.org/transmodel/journeys#VehicleJourney"/>
        <rdfs:comment xml:lang="en">A Service Journey is served by Vehicle Journeys</rdfs:comment>
        <rdfs:label xml:lang="en">service Journey Served By Vehicle Journey</rdfs:label>
    </owl:ObjectProperty>
    


    <!-- https://w3id.org/transmodel/organisations#trip -->

    <owl:ObjectProperty rdf:about="https://w3id.org/transmodel/organisations#trip">
        <rdfs:subPropertyOf rdf:resource="https://w3id.org/transmodel/journeys#PROPS-TO-REVIEW"/>
        <rdfs:domain rdf:resource="https://w3id.org/transmodel/journeys#Trip"/>
        <rdfs:range rdf:resource="https://w3id.org/transmodel/journeys#ServiceJourney"/>
        <rdfs:comment xml:lang="en">A Trip is made of ServiceJourneys</rdfs:comment>
        <rdfs:label xml:lang="en">trip</rdfs:label>
    </owl:ObjectProperty>
    


    <!-- 
    ///////////////////////////////////////////////////////////////////////////////////////
    //
    // Data properties
    //
    ///////////////////////////////////////////////////////////////////////////////////////
     -->

    


    <!-- https://w3id.org/transmodel/commons#borderCrossing -->

    <owl:DatatypeProperty rdf:about="https://w3id.org/transmodel/commons#borderCrossing"/>
    


    <!-- https://w3id.org/transmodel/journeys#DATA-PROPERTIES-TO-REVIEW -->

    <owl:DatatypeProperty rdf:about="https://w3id.org/transmodel/journeys#DATA-PROPERTIES-TO-REVIEW"/>
    


    <!-- https://w3id.org/transmodel/journeys#arrivalDayOffset -->

    <owl:DatatypeProperty rdf:about="https://w3id.org/transmodel/journeys#arrivalDayOffset">
        <rdfs:range rdf:resource="http://www.w3.org/2001/XMLSchema#time"/>
        <rdfs:comment xml:lang="en">Arrival Day Offset (e.g., for a TimeTabledPassingTime)</rdfs:comment>
        <rdfs:label xml:lang="en">arrival day offset</rdfs:label>
    </owl:DatatypeProperty>
    


    <!-- https://w3id.org/transmodel/journeys#arrivalTime -->

    <owl:DatatypeProperty rdf:about="https://w3id.org/transmodel/journeys#arrivalTime">
        <rdfs:range rdf:resource="http://www.w3.org/2001/XMLSchema#time"/>
        <rdfs:comment xml:lang="en">Arrival time (e.g., for a Service Journey in a Timing Point)</rdfs:comment>
        <rdfs:label xml:lang="en">arrival Time</rdfs:label>
    </owl:DatatypeProperty>
    


    <!-- https://w3id.org/transmodel/journeys#changeOfDestinationDisplay -->

    <owl:DatatypeProperty rdf:about="https://w3id.org/transmodel/journeys#changeOfDestinationDisplay">
        <rdfs:subPropertyOf rdf:resource="http://www.w3.org/2002/07/owl#topDataProperty"/>
        <rdfs:domain rdf:resource="https://w3id.org/transmodel/journeys#StopPointInJourneyPattern"/>
        <rdfs:range rdf:resource="http://www.w3.org/2001/XMLSchema#boolean"/>
        <rdfs:comment xml:lang="en">This property allows describing whether there will be a change of the destination display at this point</rdfs:comment>
        <rdfs:label xml:lang="en">change Of Destination Display</rdfs:label>
    </owl:DatatypeProperty>
    


    <!-- https://w3id.org/transmodel/journeys#changeOfServiceRequirements -->

    <owl:DatatypeProperty rdf:about="https://w3id.org/transmodel/journeys#changeOfServiceRequirements">
        <rdfs:subPropertyOf rdf:resource="http://www.w3.org/2002/07/owl#topDataProperty"/>
        <rdfs:domain rdf:resource="https://w3id.org/transmodel/journeys#StopPointInJourneyPattern"/>
        <rdfs:range rdf:resource="http://www.w3.org/2001/XMLSchema#boolean"/>
        <rdfs:comment xml:lang="en">This property allows describing whether there will be a change of the service requirements at this point</rdfs:comment>
        <rdfs:label xml:lang="en">change Of Service Requirements</rdfs:label>
    </owl:DatatypeProperty>
    


    <!-- https://w3id.org/transmodel/journeys#date -->

    <owl:DatatypeProperty rdf:about="https://w3id.org/transmodel/journeys#date">
        <rdfs:subPropertyOf rdf:resource="http://www.w3.org/2002/07/owl#topDataProperty"/>
        <rdfs:domain rdf:resource="https://w3id.org/transmodel/journeys#DayTypeAssignment"/>
        <rdfs:range rdf:resource="http://www.w3.org/2001/XMLSchema#dateTimeStamp"/>
        <rdfs:comment xml:lang="en">This property sets up the date for the Day Type Assignment</rdfs:comment>
        <rdfs:label xml:lang="en">date</rdfs:label>
    </owl:DatatypeProperty>
    


    <!-- https://w3id.org/transmodel/journeys#departureDayOffset -->

    <owl:DatatypeProperty rdf:about="https://w3id.org/transmodel/journeys#departureDayOffset">
        <rdfs:range rdf:resource="http://www.w3.org/2001/XMLSchema#time"/>
        <rdfs:comment xml:lang="en">Departure Day Offset (e.g., for a TimeTabledPassingTime)</rdfs:comment>
        <rdfs:label xml:lang="en">departure day offset</rdfs:label>
    </owl:DatatypeProperty>
    


    <!-- https://w3id.org/transmodel/journeys#departureTime -->

    <owl:DatatypeProperty rdf:about="https://w3id.org/transmodel/journeys#departureTime">
        <rdfs:range rdf:resource="http://www.w3.org/2001/XMLSchema#time"/>
        <rdfs:comment xml:lang="en">Departure Time (e.g., for a Service Journey in a Timing Point)</rdfs:comment>
        <rdfs:label xml:lang="en">departure Time</rdfs:label>
    </owl:DatatypeProperty>
    


    <!-- https://w3id.org/transmodel/journeys#distanceFromStart -->

    <owl:DatatypeProperty rdf:about="https://w3id.org/transmodel/journeys#distanceFromStart">
        <rdfs:range rdf:resource="http://www.w3.org/2001/XMLSchema#float"/>
        <rdfs:comment xml:lang="en">For a Point in a Link Sequence (or alike), this property represents the distance from the start of the corresponding Journey Pattern or alike.</rdfs:comment>
        <rdfs:label xml:lang="en">distance from start</rdfs:label>
    </owl:DatatypeProperty>
    


    <!-- https://w3id.org/transmodel/journeys#firstDayOffset -->

    <owl:DatatypeProperty rdf:about="https://w3id.org/transmodel/journeys#firstDayOffset">
        <rdfs:domain rdf:resource="https://w3id.org/transmodel/journeys#JourneyFrequencyGroup"/>
        <rdfs:range rdf:resource="http://www.w3.org/2001/XMLSchema#integer"/>
        <rdfs:comment xml:lang="en">offset of end time date from start time. In TransModel, there is only a day offset specified.</rdfs:comment>
        <rdfs:label xml:lang="en">first day offset</rdfs:label>
    </owl:DatatypeProperty>
    


    <!-- https://w3id.org/transmodel/journeys#firstDepartureTime -->

    <owl:DatatypeProperty rdf:about="https://w3id.org/transmodel/journeys#firstDepartureTime">
        <rdfs:domain rdf:resource="https://w3id.org/transmodel/journeys#JourneyFrequencyGroup"/>
        <rdfs:range rdf:resource="http://www.w3.org/2001/XMLSchema#time"/>
        <rdfs:comment xml:lang="en">Time of the first departure in a Journey Frequency Group</rdfs:comment>
        <rdfs:label xml:lang="en">first departure time</rdfs:label>
    </owl:DatatypeProperty>
    


    <!-- https://w3id.org/transmodel/journeys#forAlighting -->

    <owl:DatatypeProperty rdf:about="https://w3id.org/transmodel/journeys#forAlighting">
        <rdfs:subPropertyOf rdf:resource="http://www.w3.org/2002/07/owl#topDataProperty"/>
        <rdfs:domain rdf:resource="https://w3id.org/transmodel/journeys#StopPointInJourneyPattern"/>
        <rdfs:range rdf:resource="http://www.w3.org/2001/XMLSchema#boolean"/>
        <rdfs:comment xml:lang="en">This property allows describing whether the stop may be used for alighting</rdfs:comment>
        <rdfs:label xml:lang="en">for Alighting</rdfs:label>
    </owl:DatatypeProperty>
    


    <!-- https://w3id.org/transmodel/journeys#forBoarding -->

    <owl:DatatypeProperty rdf:about="https://w3id.org/transmodel/journeys#forBoarding">
        <rdfs:subPropertyOf rdf:resource="http://www.w3.org/2002/07/owl#topDataProperty"/>
        <rdfs:domain rdf:resource="https://w3id.org/transmodel/journeys#StopPointInJourneyPattern"/>
        <rdfs:range rdf:resource="http://www.w3.org/2001/XMLSchema#boolean"/>
        <rdfs:comment xml:lang="en">This property allows describing whether the stop may be used for boarding</rdfs:comment>
        <rdfs:label xml:lang="en">for Boarding</rdfs:label>
    </owl:DatatypeProperty>
    


    <!-- https://w3id.org/transmodel/journeys#headway -->

    <owl:DatatypeProperty rdf:about="https://w3id.org/transmodel/journeys#headway">
        <rdfs:subPropertyOf rdf:resource="https://w3id.org/transmodel/journeys#DATA-PROPERTIES-TO-REVIEW"/>
        <rdfs:domain rdf:resource="https://w3id.org/transmodel/journeys#JourneyPattern"/>
        <rdfs:domain rdf:resource="https://w3id.org/transmodel/journeys#VehicleJourney"/>
        <rdfs:range rdf:resource="http://www.w3.org/2001/XMLSchema#dateTimeStamp"/>
        <rdfs:label xml:lang="en">headway</rdfs:label>
    </owl:DatatypeProperty>
    


    <!-- https://w3id.org/transmodel/journeys#holidayType-old -->

    <owl:DatatypeProperty rdf:about="https://w3id.org/transmodel/journeys#holidayType-old">
        <rdfs:subPropertyOf rdf:resource="http://www.w3.org/2002/07/owl#topDataProperty"/>
        <rdfs:domain rdf:resource="https://w3id.org/transmodel/journeys#OperatingPeriod"/>
        <rdfs:comment xml:lang="en">TODO: In journeys/daytype-properties there is the top concept holiday-type which must be the skos:Concept range of this property</rdfs:comment>
        <rdfs:comment xml:lang="en">TODO: It is also a property of PropertyOfDay</rdfs:comment>
        <rdfs:comment xml:lang="en">This propery defines the type of holiday of the Operating Period</rdfs:comment>
        <rdfs:label xml:lang="en">holiday Type</rdfs:label>
    </owl:DatatypeProperty>
    


    <!-- https://w3id.org/transmodel/journeys#isAvailable -->

    <owl:DatatypeProperty rdf:about="https://w3id.org/transmodel/journeys#isAvailable">
        <rdfs:subPropertyOf rdf:resource="http://www.w3.org/2002/07/owl#topDataProperty"/>
        <rdfs:domain rdf:resource="https://w3id.org/transmodel/journeys#DayTypeAssignment"/>
        <rdfs:range rdf:resource="http://www.w3.org/2001/XMLSchema#boolean"/>
        <rdfs:comment xml:lang="en">This property says if a Day Type Assignment is available or not</rdfs:comment>
        <rdfs:label xml:lang="en">is Available</rdfs:label>
    </owl:DatatypeProperty>
    


    <!-- https://w3id.org/transmodel/journeys#isFlexible -->

    <owl:DatatypeProperty rdf:about="https://w3id.org/transmodel/journeys#isFlexible">
        <rdfs:domain rdf:resource="https://w3id.org/transmodel/journeys#StopPointInJourneyPattern"/>
        <rdfs:range rdf:resource="http://www.w3.org/2001/XMLSchema#boolean"/>
        <rdfs:comment xml:lang="en">This property is associated to a Stop Point in Journey Pattern to represent whether it is a flexible stop or not</rdfs:comment>
        <rdfs:label xml:lang="en">is flexible</rdfs:label>
    </owl:DatatypeProperty>
    


    <!-- https://w3id.org/transmodel/journeys#isServiceDay -->

    <owl:DatatypeProperty rdf:about="https://w3id.org/transmodel/journeys#isServiceDay">
        <rdfs:domain rdf:resource="https://w3id.org/transmodel/journeys#OrganisationDayType"/>
        <rdfs:range rdf:resource="http://www.w3.org/2001/XMLSchema#boolean"/>
        <rdfs:label xml:lang="en">Property that indicates whether a Transport Service is required for an Organisation on this Day Type.</rdfs:label>
        <rdfs:label xml:lang="en">is service day</rdfs:label>
    </owl:DatatypeProperty>
    


    <!-- https://w3id.org/transmodel/journeys#isWaitPoint -->

    <owl:DatatypeProperty rdf:about="https://w3id.org/transmodel/journeys#isWaitPoint">
        <rdfs:subPropertyOf rdf:resource="http://www.w3.org/2002/07/owl#topDataProperty"/>
        <rdf:type rdf:resource="http://www.w3.org/2002/07/owl#FunctionalProperty"/>
        <rdfs:domain rdf:resource="https://w3id.org/transmodel/journeys#TimingPointInJourneyPattern"/>
        <rdfs:range rdf:resource="http://www.w3.org/2001/XMLSchema#boolean"/>
        <rdfs:comment xml:lang="en">This property allows describing whether a Timing Point is a wait point</rdfs:comment>
        <rdfs:label xml:lang="en">is Wait Point</rdfs:label>
    </owl:DatatypeProperty>
    


    <!-- https://w3id.org/transmodel/journeys#lastDayOffset -->

    <owl:DatatypeProperty rdf:about="https://w3id.org/transmodel/journeys#lastDayOffset">
        <rdfs:domain rdf:resource="https://w3id.org/transmodel/journeys#JourneyFrequencyGroup"/>
        <rdfs:range rdf:resource="http://www.w3.org/2001/XMLSchema#integer"/>
        <rdfs:comment xml:lang="en">Offset of end time date from start time. In TransModel, there is only a day offset specified.</rdfs:comment>
        <rdfs:label xml:lang="en">last day offset</rdfs:label>
    </owl:DatatypeProperty>
    


    <!-- https://w3id.org/transmodel/journeys#lastDepartureTime -->

    <owl:DatatypeProperty rdf:about="https://w3id.org/transmodel/journeys#lastDepartureTime">
        <rdfs:domain rdf:resource="https://w3id.org/transmodel/journeys#JourneyFrequencyGroup"/>
        <rdfs:range rdf:resource="http://www.w3.org/2001/XMLSchema#time"/>
        <rdfs:comment xml:lang="en">Time of the last departure in a Journey Frequency Group</rdfs:comment>
        <rdfs:label xml:lang="en">last departure time</rdfs:label>
    </owl:DatatypeProperty>
    


    <!-- https://w3id.org/transmodel/journeys#layover -->

    <owl:DatatypeProperty rdf:about="https://w3id.org/transmodel/journeys#layover">
        <rdfs:subPropertyOf rdf:resource="https://w3id.org/transmodel/journeys#DATA-PROPERTIES-TO-REVIEW"/>
        <rdfs:domain rdf:resource="https://w3id.org/transmodel/journeys#JourneyPattern"/>
        <rdfs:domain rdf:resource="https://w3id.org/transmodel/journeys#VehicleJourney"/>
        <rdfs:range rdf:resource="http://www.w3.org/2001/XMLSchema#dateTimeStamp"/>
        <rdfs:label xml:lang="en">layover</rdfs:label>
    </owl:DatatypeProperty>
    


    <!-- https://w3id.org/transmodel/journeys#lineName -->

    <owl:DatatypeProperty rdf:about="https://w3id.org/transmodel/journeys#lineName">
        <rdfs:subPropertyOf rdf:resource="https://w3id.org/transmodel/journeys#DATA-PROPERTIES-TO-REVIEW"/>
        <rdfs:domain rdf:resource="https://w3id.org/transmodel/journeys#Line-old"/>
        <rdfs:range rdf:resource="http://www.w3.org/2000/01/rdf-schema#Literal"/>
        <rdfs:label xml:lang="en">lineName</rdfs:label>
    </owl:DatatypeProperty>
    


    <!-- https://w3id.org/transmodel/journeys#lineNumber -->

    <owl:DatatypeProperty rdf:about="https://w3id.org/transmodel/journeys#lineNumber">
        <rdfs:subPropertyOf rdf:resource="https://w3id.org/transmodel/journeys#DATA-PROPERTIES-TO-REVIEW"/>
        <rdfs:domain rdf:resource="https://w3id.org/transmodel/journeys#Line-old"/>
        <rdfs:range rdf:resource="http://www.w3.org/2001/XMLSchema#nonNegativeInteger"/>
        <rdfs:label xml:lang="en">lineNumber</rdfs:label>
    </owl:DatatypeProperty>
    


    <!-- https://w3id.org/transmodel/journeys#maximumHeadwayInterval -->

    <owl:DatatypeProperty rdf:about="https://w3id.org/transmodel/journeys#maximumHeadwayInterval">
        <rdfs:domain rdf:resource="https://w3id.org/transmodel/journeys#HeadwayInterval"/>
        <rdfs:range rdf:resource="http://www.w3.org/2001/XMLSchema#duration"/>
        <rdfs:comment xml:lang="en">Maximum headway interval for a Headway Interval of a Headway Journey Group.</rdfs:comment>
        <rdfs:label xml:lang="en">maximum headway interval</rdfs:label>
    </owl:DatatypeProperty>
    


    <!-- https://w3id.org/transmodel/journeys#minimumHeadwayInterval -->

    <owl:DatatypeProperty rdf:about="https://w3id.org/transmodel/journeys#minimumHeadwayInterval">
        <rdfs:domain rdf:resource="https://w3id.org/transmodel/journeys#HeadwayInterval"/>
        <rdfs:range rdf:resource="http://www.w3.org/2001/XMLSchema#duration"/>
        <rdfs:comment xml:lang="en">Minimum headway interval for a Headway Interval of a Headway Journey Group.</rdfs:comment>
        <rdfs:label xml:lang="en">minimum headway interval</rdfs:label>
    </owl:DatatypeProperty>
    


    <!-- https://w3id.org/transmodel/journeys#monitored -->

    <owl:DatatypeProperty rdf:about="https://w3id.org/transmodel/journeys#monitored">
        <rdfs:subPropertyOf rdf:resource="http://www.w3.org/2002/07/owl#topDataProperty"/>
        <rdfs:domain rdf:resource="https://w3id.org/transmodel/journeys#Journey"/>
        <rdfs:range rdf:resource="http://www.w3.org/2001/XMLSchema#boolean"/>
        <rdfs:comment xml:lang="en">This property defines whether the journey is monitored or not</rdfs:comment>
        <rdfs:label xml:lang="en">monitored</rdfs:label>
    </owl:DatatypeProperty>
    


    <!-- https://w3id.org/transmodel/journeys#order -->

    <owl:DatatypeProperty rdf:about="https://w3id.org/transmodel/journeys#order">
        <rdfs:subPropertyOf rdf:resource="http://www.w3.org/2002/07/owl#topDataProperty"/>
        <rdfs:range rdf:resource="http://www.w3.org/2001/XMLSchema#nonNegativeInteger"/>
        <rdfs:comment xml:lang="en">Order of a Point in Link Sequence, or in a Point on Route within sequence, or in any other type of situation where the order or points are relevant</rdfs:comment>
        <rdfs:label xml:lang="en">order</rdfs:label>
    </owl:DatatypeProperty>
    


    <!-- https://w3id.org/transmodel/journeys#requestStop -->

    <owl:DatatypeProperty rdf:about="https://w3id.org/transmodel/journeys#requestStop">
        <rdfs:subPropertyOf rdf:resource="http://www.w3.org/2002/07/owl#topDataProperty"/>
        <rdfs:domain rdf:resource="https://w3id.org/transmodel/journeys#StopPointInJourneyPattern"/>
        <rdfs:range rdf:resource="http://www.w3.org/2001/XMLSchema#boolean"/>
        <rdfs:comment xml:lang="en">This property allows describing whether the stop is a Request Stop</rdfs:comment>
        <rdfs:label xml:lang="en">request Stop</rdfs:label>
    </owl:DatatypeProperty>
    


    <!-- https://w3id.org/transmodel/journeys#runtime -->

    <owl:DatatypeProperty rdf:about="https://w3id.org/transmodel/journeys#runtime">
        <rdfs:subPropertyOf rdf:resource="https://w3id.org/transmodel/journeys#DATA-PROPERTIES-TO-REVIEW"/>
        <rdfs:domain rdf:resource="https://w3id.org/transmodel/journeys#JourneyPattern"/>
        <rdfs:domain rdf:resource="https://w3id.org/transmodel/journeys#VehicleJourney"/>
        <rdfs:range rdf:resource="http://www.w3.org/2001/XMLSchema#nonNegativeInteger"/>
        <rdfs:label xml:lang="en">runtime</rdfs:label>
    </owl:DatatypeProperty>
    


    <!-- https://w3id.org/transmodel/journeys#scheduledHeadwayInterval -->

    <owl:DatatypeProperty rdf:about="https://w3id.org/transmodel/journeys#scheduledHeadwayInterval">
        <rdfs:domain rdf:resource="https://w3id.org/transmodel/journeys#HeadwayInterval"/>
        <rdfs:range rdf:resource="http://www.w3.org/2001/XMLSchema#duration"/>
        <rdfs:comment xml:lang="en">Scheduled headway interval for a Headway Interval of a Headway Journey Group.</rdfs:comment>
        <rdfs:label xml:lang="en">scheduled headway interval</rdfs:label>
    </owl:DatatypeProperty>
    


    <!-- https://w3id.org/transmodel/journeys#startTime -->

    <owl:DatatypeProperty rdf:about="https://w3id.org/transmodel/journeys#startTime">
        <rdfs:subPropertyOf rdf:resource="https://w3id.org/transmodel/journeys#DATA-PROPERTIES-TO-REVIEW"/>
        <rdfs:range rdf:resource="http://www.w3.org/2001/XMLSchema#string"/>
        <rdfs:label xml:lang="en">startTime</rdfs:label>
    </owl:DatatypeProperty>
    


    <!-- https://w3id.org/transmodel/journeys#time -->

    <owl:DatatypeProperty rdf:about="https://w3id.org/transmodel/journeys#time">
        <rdfs:subPropertyOf rdf:resource="https://w3id.org/transmodel/journeys#DATA-PROPERTIES-TO-REVIEW"/>
        <rdfs:domain rdf:resource="https://w3id.org/transmodel/journeys#JourneyPatternLayover"/>
        <rdfs:domain rdf:resource="https://w3id.org/transmodel/journeys#TimingPoint"/>
        <rdfs:domain rdf:resource="https://w3id.org/transmodel/journeys#VehicleJourneyLayover"/>
        <rdfs:range rdf:resource="http://www.w3.org/2001/XMLSchema#dateTimeStamp"/>
        <rdfs:label xml:lang="en">time</rdfs:label>
    </owl:DatatypeProperty>
    


    <!-- https://w3id.org/transmodel/journeys#timeLink -->

    <owl:DatatypeProperty rdf:about="https://w3id.org/transmodel/journeys#timeLink">
        <rdfs:subPropertyOf rdf:resource="https://w3id.org/transmodel/journeys#DATA-PROPERTIES-TO-REVIEW"/>
        <rdfs:domain rdf:resource="https://w3id.org/transmodel/journeys#TimingPoint"/>
        <rdfs:range rdf:resource="http://www.w3.org/2001/XMLSchema#nonNegativeInteger"/>
        <rdfs:comment xml:lang="en">Sequences of TimePoints</rdfs:comment>
        <rdfs:label xml:lang="en">timeLink</rdfs:label>
    </owl:DatatypeProperty>
    


    <!-- https://w3id.org/transmodel/journeys#timingLinkInJourneyPattern -->

    <owl:DatatypeProperty rdf:about="https://w3id.org/transmodel/journeys#timingLinkInJourneyPattern">
        <rdfs:subPropertyOf rdf:resource="https://w3id.org/transmodel/journeys#DATA-PROPERTIES-TO-REVIEW"/>
    </owl:DatatypeProperty>
    


    <!-- https://w3id.org/transmodel/journeys#timingLinkPointSequence -->

    <owl:DatatypeProperty rdf:about="https://w3id.org/transmodel/journeys#timingLinkPointSequence">
        <rdfs:subPropertyOf rdf:resource="https://w3id.org/transmodel/journeys#DATA-PROPERTIES-TO-REVIEW"/>
        <rdfs:domain rdf:resource="https://w3id.org/transmodel/journeys#TimingPoint"/>
        <rdfs:range rdf:resource="http://www.w3.org/2001/XMLSchema#nonNegativeInteger"/>
    </owl:DatatypeProperty>
    


    <!-- https://w3id.org/transmodel/journeys#viaFlag -->

    <owl:DatatypeProperty rdf:about="https://w3id.org/transmodel/journeys#viaFlag">
        <rdfs:domain rdf:resource="https://w3id.org/transmodel/journeys#RoutePoint"/>
        <rdfs:range rdf:resource="http://www.w3.org/2001/XMLSchema#boolean"/>
        <rdfs:comment xml:lang="en">This property detemines whether a Route Point is flagged as a via point</rdfs:comment>
        <rdfs:label xml:lang="en">via flag</rdfs:label>
    </owl:DatatypeProperty>
    


    <!-- https://w3id.org/transmodel/journeys#waitTime -->

    <owl:DatatypeProperty rdf:about="https://w3id.org/transmodel/journeys#waitTime">
        <rdfs:subPropertyOf rdf:resource="https://w3id.org/transmodel/journeys#DATA-PROPERTIES-TO-REVIEW"/>
        <rdfs:domain rdf:resource="https://w3id.org/transmodel/journeys#JourneyPattern"/>
        <rdfs:domain rdf:resource="https://w3id.org/transmodel/journeys#VehicleJourney"/>
        <rdfs:range rdf:resource="http://www.w3.org/2001/XMLSchema#string"/>
        <rdfs:label xml:lang="en">waitTime</rdfs:label>
    </owl:DatatypeProperty>
    


    <!-- 
    ///////////////////////////////////////////////////////////////////////////////////////
    //
    // Classes
    //
    ///////////////////////////////////////////////////////////////////////////////////////
     -->

    


    <!-- http://www.w3.org/2004/02/skos/core#Concept -->

    <owl:Class rdf:about="http://www.w3.org/2004/02/skos/core#Concept"/>
    


    <!-- http://www.w3.org/2004/02/skos/core#ConceptScheme -->

    <owl:Class rdf:about="http://www.w3.org/2004/02/skos/core#ConceptScheme"/>
    


    <!-- https://w3id.org/transmodel/commons#Presentation -->

    <owl:Class rdf:about="https://w3id.org/transmodel/commons#Presentation"/>
    


    <!-- https://w3id.org/transmodel/facilities#AccessibilityAssessment -->

    <owl:Class rdf:about="https://w3id.org/transmodel/facilities#AccessibilityAssessment">
        <rdfs:label xml:lang="en">Accessibility Assessment</rdfs:label>
    </owl:Class>
    


    <!-- https://w3id.org/transmodel/facilities#BoardingPosition -->

    <owl:Class rdf:about="https://w3id.org/transmodel/facilities#BoardingPosition"/>
    


    <!-- https://w3id.org/transmodel/facilities#JourneyPattern -->

    <owl:Class rdf:about="https://w3id.org/transmodel/facilities#JourneyPattern">
        <rdfs:subClassOf rdf:resource="https://w3id.org/transmodel/journeys#TOREVIEWCLASSES"/>
    </owl:Class>
    


    <!-- https://w3id.org/transmodel/facilities#Quay -->

    <owl:Class rdf:about="https://w3id.org/transmodel/facilities#Quay"/>
    


    <!-- https://w3id.org/transmodel/facilities#ServiceFacilitySet -->

    <owl:Class rdf:about="https://w3id.org/transmodel/facilities#ServiceFacilitySet">
        <rdfs:subClassOf>
            <owl:Restriction>
                <owl:onProperty rdf:resource="https://w3id.org/transmodel/journeys#madeUsing"/>
                <owl:allValuesFrom rdf:resource="https://w3id.org/transmodel/facilities#ServiceFacilitySet"/>
            </owl:Restriction>
        </rdfs:subClassOf>
        <rdfs:label xml:lang="en">Service Facility Set</rdfs:label>
    </owl:Class>
    


    <!-- https://w3id.org/transmodel/facilities#StopPlace -->

    <owl:Class rdf:about="https://w3id.org/transmodel/facilities#StopPlace"/>
    


    <!-- https://w3id.org/transmodel/facilities#VehicleType -->

    <owl:Class rdf:about="https://w3id.org/transmodel/facilities#VehicleType">
        <rdfs:comment xml:lang="en">A classification of public transport vehicles according to the vehicle scheduling requirements in mode and capacity (e.g. standard bus, double-deck, ...).</rdfs:comment>
        <rdfs:label xml:lang="en">Vehicle Type</rdfs:label>
    </owl:Class>
    


    <!-- https://w3id.org/transmodel/journeys#Access -->

    <owl:Class rdf:about="https://w3id.org/transmodel/journeys#Access">
        <rdfs:subClassOf rdf:resource="https://w3id.org/transmodel/journeys#TOREVIEWCLASSES"/>
        <rdfs:comment xml:lang="en">The physical spatial possibility for a passenger to access or leave the public transport system. The link may be used during a Trip for:

- The walking movement of the Passenger from a Place (Origin of the Trip) to a ScheduledStopPoint (origin of the Public Transport Trip).
- The walking movement of the Passenger from a Scheduled Stop Point (destination of the Public Transport Trip) to a Place (destination of the Trip)</rdfs:comment>
        <rdfs:label xml:lang="en">TypeOfAccess</rdfs:label>
    </owl:Class>
    


    <!-- https://w3id.org/transmodel/journeys#AccessMode -->

    <owl:Class rdf:about="https://w3id.org/transmodel/journeys#AccessMode">
        <rdfs:subClassOf rdf:resource="https://w3id.org/transmodel/journeys#TOREVIEWCLASSES"/>
        <rdfs:comment xml:lang="en">A characterisation of the passenger movement according to the means of transport different from public transport: walking, own bike,</rdfs:comment>
        <rdfs:label xml:lang="en">AccessMode</rdfs:label>
    </owl:Class>
    


    <!-- https://w3id.org/transmodel/journeys#AccessZone -->

    <owl:Class rdf:about="https://w3id.org/transmodel/journeys#AccessZone">
        <rdfs:subClassOf rdf:resource="https://w3id.org/transmodel/journeys#TOREVIEWCLASSES"/>
        <rdfs:comment xml:lang="en">A Zone for which the duration to cover any Access link to a particular ScheduledStopPoint is the same</rdfs:comment>
        <rdfs:label xml:lang="en">AccessZone</rdfs:label>
    </owl:Class>
    


    <!-- https://w3id.org/transmodel/journeys#ActivationPoint -->

    <owl:Class rdf:about="https://w3id.org/transmodel/journeys#ActivationPoint">
        <rdfs:subClassOf rdf:resource="https://w3id.org/transmodel/journeys#Point"/>
        <rdfs:comment xml:lang="en">A Point where a control process is activated when a vehicle passes it. Equipment may be needed for the activation.</rdfs:comment>
        <rdfs:comment xml:lang="en">TODO: Complete with all relevant properties</rdfs:comment>
        <rdfs:label xml:lang="en">Activation Point</rdfs:label>
    </owl:Class>
    


    <!-- https://w3id.org/transmodel/journeys#Address -->

    <owl:Class rdf:about="https://w3id.org/transmodel/journeys#Address">
        <rdfs:subClassOf rdf:resource="https://w3id.org/transmodel/journeys#TOREVIEWCLASSES"/>
        <rdfs:comment xml:lang="en">The descriptive data associated with a Place that can be used to describe the unique geographical context of a Place for the purposes of identifying. May be refined as either a Road Address, a Postal Address or both.</rdfs:comment>
        <rdfs:label xml:lang="en">Address</rdfs:label>
    </owl:Class>
    


    <!-- https://w3id.org/transmodel/journeys#AddressablePlace -->

    <owl:Class rdf:about="https://w3id.org/transmodel/journeys#AddressablePlace">
        <rdfs:subClassOf rdf:resource="https://w3id.org/transmodel/journeys#Place"/>
        <rdfs:comment xml:lang="en">A type of Place to which Passengers may refer to indicate the origin or a destination of a trip and that is so specific that it has an Address.</rdfs:comment>
        <rdfs:label xml:lang="en">AddressablePlace</rdfs:label>
    </owl:Class>
    


    <!-- https://w3id.org/transmodel/journeys#AllowedLineDirections -->

    <owl:Class rdf:about="https://w3id.org/transmodel/journeys#AllowedLineDirections">
        <rdfs:subClassOf rdf:resource="https://w3id.org/transmodel/journeys#TOREVIEWCLASSES"/>
        <rdfs:comment xml:lang="en">An allowed direction that can be used on a given Route. This can be used to validate the selection of allowed values</rdfs:comment>
        <rdfs:label xml:lang="en">AllowedLineDirections</rdfs:label>
    </owl:Class>
    


    <!-- https://w3id.org/transmodel/journeys#BeaconPoint -->

    <owl:Class rdf:about="https://w3id.org/transmodel/journeys#BeaconPoint">
        <rdfs:subClassOf rdf:resource="https://w3id.org/transmodel/journeys#Point"/>
        <rdfs:comment xml:lang="en">A Point where a beacon or similar device to support the automatic detection of Vehicles passing by is located</rdfs:comment>
        <rdfs:label xml:lang="en">BeaconPoint</rdfs:label>
    </owl:Class>
    


    <!-- https://w3id.org/transmodel/journeys#Block -->

    <owl:Class rdf:about="https://w3id.org/transmodel/journeys#Block">
        <rdfs:comment xml:lang="en">The work of a vehicle from the time it leaves a Parking Point after parking until its next return to park at a Parking Point. Any subsequent departure from a Parking Point after parking marks the start of a new Block. The period of a Block must be covered by Duties.</rdfs:comment>
        <rdfs:label xml:lang="en">Block</rdfs:label>
    </owl:Class>
    


    <!-- https://w3id.org/transmodel/journeys#BlockPart -->

    <owl:Class rdf:about="https://w3id.org/transmodel/journeys#BlockPart">
        <rdfs:subClassOf rdf:resource="https://w3id.org/transmodel/journeys#TOREVIEWCLASSES"/>
        <rdfs:comment xml:lang="en">Part of a Block corresponding to the different JourneyPart of the VehicleJourney in a Block</rdfs:comment>
        <rdfs:label xml:lang="en">BlockPart</rdfs:label>
    </owl:Class>
    


    <!-- https://w3id.org/transmodel/journeys#BoardingPosition -->

    <owl:Class rdf:about="https://w3id.org/transmodel/journeys#BoardingPosition">
        <rdfs:comment xml:lang="en">A location within a Quay from which Passenger may directly board, or onto which passengers may directly alight from a Vehicle</rdfs:comment>
        <rdfs:label xml:lang="en">Boarding Position</rdfs:label>
    </owl:Class>
    


    <!-- https://w3id.org/transmodel/journeys#CompoundBlock -->

    <owl:Class rdf:about="https://w3id.org/transmodel/journeys#CompoundBlock">
        <rdfs:subClassOf rdf:resource="https://w3id.org/transmodel/journeys#TOREVIEWCLASSES"/>
        <rdfs:comment xml:lang="en">The work of a vehicle during the time it is coupled to anohter vehicle</rdfs:comment>
        <rdfs:label xml:lang="en">CompoundBlock</rdfs:label>
    </owl:Class>
    


    <!-- https://w3id.org/transmodel/journeys#Connection -->

    <owl:Class rdf:about="https://w3id.org/transmodel/journeys#Connection">
        <rdfs:subClassOf rdf:resource="https://w3id.org/transmodel/journeys#TOREVIEWCLASSES"/>
        <rdfs:comment xml:lang="en">The physical (spatial) possibility for a Passenger to change from one public transport vehicle to another to continue the trip, determined by two ScheduledStopPoint. Different times may be necessary to cover the link between these points, depending the kind of Passenger</rdfs:comment>
        <rdfs:label xml:lang="en">Connection</rdfs:label>
    </owl:Class>
    


    <!-- https://w3id.org/transmodel/journeys#CoupledJourney -->

    <owl:Class rdf:about="https://w3id.org/transmodel/journeys#CoupledJourney">
        <rdfs:subClassOf rdf:resource="https://w3id.org/transmodel/journeys#TOREVIEWCLASSES"/>
        <rdfs:comment xml:lang="en">A complete journey operated by a coupled train, composed of two or more Vehicle Journeys remaining coupled together all along a Journey Pattern. A Coupled Journey may be viewed as a single VehicleJourney.</rdfs:comment>
        <rdfs:label xml:lang="en">CoupledJourney</rdfs:label>
    </owl:Class>
    


    <!-- https://w3id.org/transmodel/journeys#CourseOfJourneys -->

    <owl:Class rdf:about="https://w3id.org/transmodel/journeys#CourseOfJourneys">
        <rdfs:subClassOf rdf:resource="https://w3id.org/transmodel/journeys#TOREVIEWCLASSES"/>
        <rdfs:comment xml:lang="en">A part of a Block composed of consecutive VehicleJourneys defined for the same DayType, all operated on the same Line.</rdfs:comment>
        <rdfs:label xml:lang="en">CourseOfJourneys</rdfs:label>
    </owl:Class>
    


    <!-- https://w3id.org/transmodel/journeys#DatedBlock -->

    <owl:Class rdf:about="https://w3id.org/transmodel/journeys#DatedBlock">
        <rdfs:subClassOf rdf:resource="https://w3id.org/transmodel/journeys#Block"/>
        <rdfs:comment xml:lang="en">The work of a Vehicle on a particular Operating Day from the time it leaves a Parking Point after parking until its next return to park at a Parking Point</rdfs:comment>
        <rdfs:label xml:lang="en">DatedBlock</rdfs:label>
    </owl:Class>
    


    <!-- https://w3id.org/transmodel/journeys#DatedVehicleJourney -->

    <owl:Class rdf:about="https://w3id.org/transmodel/journeys#DatedVehicleJourney">
        <rdfs:subClassOf rdf:resource="https://w3id.org/transmodel/journeys#VehicleJourney"/>
        <rdfs:comment xml:lang="en">A particular Journey of a Vehicle on a particular OperatingDay including all modifications possibly decided by the control staff</rdfs:comment>
        <rdfs:label xml:lang="en">Dated Vehicle Journey</rdfs:label>
    </owl:Class>
    


    <!-- https://w3id.org/transmodel/journeys#DayType -->

    <owl:Class rdf:about="https://w3id.org/transmodel/journeys#DayType">
        <rdfs:subClassOf>
            <owl:Restriction>
                <owl:onProperty rdf:resource="https://w3id.org/transmodel/journeys#describedBy"/>
                <owl:allValuesFrom rdf:resource="https://w3id.org/transmodel/journeys#PropertyOfDay"/>
            </owl:Restriction>
        </rdfs:subClassOf>
        <rdfs:subClassOf>
            <owl:Restriction>
                <owl:onProperty rdf:resource="https://w3id.org/transmodel/journeys#specifying"/>
                <owl:allValuesFrom rdf:resource="https://w3id.org/transmodel/journeys#DayType"/>
            </owl:Restriction>
        </rdfs:subClassOf>
        <rdfs:subClassOf>
            <owl:Restriction>
                <owl:onProperty rdf:resource="https://w3id.org/transmodel/journeys#season"/>
                <owl:maxQualifiedCardinality rdf:datatype="http://www.w3.org/2001/XMLSchema#nonNegativeInteger">1</owl:maxQualifiedCardinality>
                <owl:onClass>
                    <owl:Class>
                        <owl:intersectionOf rdf:parseType="Collection">
                            <rdf:Description rdf:about="http://www.w3.org/2004/02/skos/core#Concept"/>
                            <owl:Restriction>
                                <owl:onProperty rdf:resource="http://www.w3.org/2004/02/skos/core#inScheme"/>
                                <owl:hasValue rdf:resource="https://w3id.org/transmodel/kos/journeys/day-type"/>
                            </owl:Restriction>
                        </owl:intersectionOf>
                    </owl:Class>
                </owl:onClass>
            </owl:Restriction>
        </rdfs:subClassOf>
        <rdfs:comment xml:lang="en">A Day Type is a type of day characterised by one or more properties which affect public transport operation</rdfs:comment>
        <rdfs:label xml:lang="en">Day Type</rdfs:label>
        <rdfs:label xml:lang="en">TODO: Check season and complete with other properties</rdfs:label>
    </owl:Class>
    


    <!-- https://w3id.org/transmodel/journeys#DayTypeAssignment -->

    <owl:Class rdf:about="https://w3id.org/transmodel/journeys#DayTypeAssignment">
        <rdfs:subClassOf>
            <owl:Restriction>
                <owl:onProperty rdf:resource="https://w3id.org/transmodel/journeys#operatingPeriod"/>
                <owl:allValuesFrom rdf:resource="https://w3id.org/transmodel/journeys#OperatingPeriod"/>
            </owl:Restriction>
        </rdfs:subClassOf>
        <rdfs:comment xml:lang="en">The assignment of operational characteristics, expressed by Day Type to particular Operating Day within a Service Calendar</rdfs:comment>
        <rdfs:label xml:lang="en">Day Type Assignment</rdfs:label>
    </owl:Class>
    


    <!-- https://w3id.org/transmodel/journeys#DeadRun -->

    <owl:Class rdf:about="https://w3id.org/transmodel/journeys#DeadRun">
        <rdfs:subClassOf rdf:resource="https://w3id.org/transmodel/journeys#VehicleJourney"/>
        <rdfs:comment xml:lang="en">A non-service VehicleJourney</rdfs:comment>
        <rdfs:label xml:lang="en">Dead Run</rdfs:label>
    </owl:Class>
    


    <!-- https://w3id.org/transmodel/journeys#DeadRunPattern -->

    <owl:Class rdf:about="https://w3id.org/transmodel/journeys#DeadRunPattern">
        <rdfs:subClassOf rdf:resource="https://w3id.org/transmodel/journeys#JourneyPattern"/>
        <rdfs:comment xml:lang="en">A JourneyPattern to be used for DeadRun</rdfs:comment>
        <rdfs:label xml:lang="en">DeadRunPattern</rdfs:label>
    </owl:Class>
    


    <!-- https://w3id.org/transmodel/journeys#DefaultConnection -->

    <owl:Class rdf:about="https://w3id.org/transmodel/journeys#DefaultConnection">
        <rdfs:subClassOf rdf:resource="https://w3id.org/transmodel/journeys#Connection"/>
        <rdfs:comment xml:lang="en">The physical (spatial) possibility for a Passenger to change from one public transport Vehicle to another to continue the Trip. It specifies default times to be used to change from one mode of transport to another at an area or national level as specified by a TopographicPlace, Stop Area or SiteElement. It may be restricted to a specific Mode or Operator oe only apply in a particular direction of transfer, e.g. bus to rail may have a different time for rail to bus.</rdfs:comment>
        <rdfs:label xml:lang="en">DefaultConnection</rdfs:label>
    </owl:Class>
    


    <!-- https://w3id.org/transmodel/journeys#DefaultDeadRunRunTime -->

    <owl:Class rdf:about="https://w3id.org/transmodel/journeys#DefaultDeadRunRunTime">
        <rdfs:subClassOf rdf:resource="https://w3id.org/transmodel/journeys#TOREVIEWCLASSES"/>
        <rdfs:label xml:lang="en">DefaultDeadRunRunTime</rdfs:label>
    </owl:Class>
    


    <!-- https://w3id.org/transmodel/journeys#DefaultInterchange -->

    <owl:Class rdf:about="https://w3id.org/transmodel/journeys#DefaultInterchange">
        <rdfs:subClassOf rdf:resource="https://w3id.org/transmodel/journeys#TOREVIEWCLASSES"/>
        <rdfs:comment xml:lang="en">A quality parameter fixing the acceptable duration (standard and maximum) for an Interchage to be planned between two ScheduledStopPoint. this parameter will be used to control whether any two VehicleJourney serving those Points may be in connection.</rdfs:comment>
        <rdfs:label xml:lang="en">DefaultInterchange</rdfs:label>
    </owl:Class>
    


    <!-- https://w3id.org/transmodel/journeys#DefaultServiceJourneyRunTime -->

    <owl:Class rdf:about="https://w3id.org/transmodel/journeys#DefaultServiceJourneyRunTime">
        <rdfs:subClassOf rdf:resource="https://w3id.org/transmodel/journeys#TOREVIEWCLASSES"/>
        <rdfs:comment xml:lang="en">The default time taken by a Vehicle to traverse a TimingLink during a ServiceJourney, for a specified TimeDemandType. This time may be superseded by the JourneyPatternRunTime or VehicleJourneyRunTime if these exist</rdfs:comment>
        <rdfs:label xml:lang="en">DefaultServiceJourneyRunTime</rdfs:label>
    </owl:Class>
    


    <!-- https://w3id.org/transmodel/journeys#DestinationDisplay -->

    <owl:Class rdf:about="https://w3id.org/transmodel/journeys#DestinationDisplay">
        <rdfs:comment xml:lang="en">An advertised destination of a specific Journey Pattern usually displayed on a headsign or other on-board locations</rdfs:comment>
        <rdfs:label xml:lang="en">Destination Display</rdfs:label>
    </owl:Class>
    


    <!-- https://w3id.org/transmodel/journeys#DestinationDisplayVariant -->

    <owl:Class rdf:about="https://w3id.org/transmodel/journeys#DestinationDisplayVariant">
        <rdfs:subClassOf rdf:resource="https://w3id.org/transmodel/journeys#DestinationDisplay"/>
        <rdfs:comment xml:lang="en">An advertised destination of a specific Journey Pattern, usually displayed on a headsign (Heading Sign) or at other on-board locations</rdfs:comment>
        <rdfs:label xml:lang="en">Destination Display Variant</rdfs:label>
    </owl:Class>
    


    <!-- https://w3id.org/transmodel/journeys#DynamicStopAssignment -->

    <owl:Class rdf:about="https://w3id.org/transmodel/journeys#DynamicStopAssignment">
        <rdfs:subClassOf rdf:resource="https://w3id.org/transmodel/journeys#PassengerStopAssignment"/>
        <rdfs:subClassOf>
            <owl:Restriction>
                <owl:onProperty rdf:resource="https://w3id.org/transmodel/journeys#overriding"/>
                <owl:allValuesFrom rdf:resource="https://w3id.org/transmodel/journeys#PassengerStopAssignment"/>
            </owl:Restriction>
        </rdfs:subClassOf>
        <rdfs:comment xml:lang="en">The dynamic association of a Scheduled Stop Point with the next available Stop Place, Quay or Boarding Position within a Stop Place.</rdfs:comment>
        <rdfs:label xml:lang="en">Dynamic Stop Assignment</rdfs:label>
    </owl:Class>
    


    <!-- https://w3id.org/transmodel/journeys#FareDayType -->

    <owl:Class rdf:about="https://w3id.org/transmodel/journeys#FareDayType">
        <rdfs:subClassOf rdf:resource="https://w3id.org/transmodel/journeys#DayType"/>
        <rdfs:comment xml:lang="en">A type of day used in the fare collection domain, characterised by one or more properties which affect the definition of access rights and prices in the fare system.</rdfs:comment>
        <rdfs:comment xml:lang="en">TODO: Add information on the relationship with PricingParameterSet</rdfs:comment>
        <rdfs:label xml:lang="en">Fare Day Type</rdfs:label>
    </owl:Class>
    


    <!-- https://w3id.org/transmodel/journeys#FarePointInJourneyPattern -->

    <owl:Class rdf:about="https://w3id.org/transmodel/journeys#FarePointInJourneyPattern">
        <rdfs:subClassOf rdf:resource="https://w3id.org/transmodel/journeys#PointInJourneyPattern"/>
        <rdfs:comment xml:lang="en">TODO: Add all relevant properties here</rdfs:comment>
        <rdfs:comment xml:lang="en">TODO: This should be probably moved to the Fares module, unless we make a link from that fares module into this one.</rdfs:comment>
    </owl:Class>
    


    <!-- https://w3id.org/transmodel/journeys#FlexibleLine -->

    <owl:Class rdf:about="https://w3id.org/transmodel/journeys#FlexibleLine">
        <rdfs:subClassOf rdf:resource="https://w3id.org/transmodel/journeys#Line-old"/>
        <rdfs:comment xml:lang="en">Specialisation of Line for FlexibleService. As all the service on a Line may not be flexible, flexibility itself is described at JourneyPattern level, meaning that a separate JourneyPattern is needed for each type of flexibility available for the Line</rdfs:comment>
        <rdfs:label xml:lang="en">FlexibleLine</rdfs:label>
    </owl:Class>
    


    <!-- https://w3id.org/transmodel/journeys#FlexiblePoint -->

    <owl:Class rdf:about="https://w3id.org/transmodel/journeys#FlexiblePoint">
        <rdfs:subClassOf rdf:resource="https://w3id.org/transmodel/journeys#Point"/>
        <rdfs:comment xml:lang="en">A specialisation of Point for Flexible Service</rdfs:comment>
        <rdfs:label xml:lang="en">Flexible Point</rdfs:label>
    </owl:Class>
    


    <!-- https://w3id.org/transmodel/journeys#FlexibleRoute -->

    <owl:Class rdf:about="https://w3id.org/transmodel/journeys#FlexibleRoute">
        <rdfs:subClassOf rdf:resource="https://w3id.org/transmodel/journeys#TOREVIEWCLASSES"/>
        <rdfs:comment xml:lang="en">Specialisation of Route for FlexibleService. May include both Point and Zonal areas and ordered and unordered sections.</rdfs:comment>
        <rdfs:label xml:lang="en">FlexibleRoute</rdfs:label>
    </owl:Class>
    


    <!-- https://w3id.org/transmodel/journeys#GaragePoint -->

    <owl:Class rdf:about="https://w3id.org/transmodel/journeys#GaragePoint">
        <rdfs:subClassOf rdf:resource="https://w3id.org/transmodel/journeys#ParkingPoint"/>
        <rdfs:comment xml:lang="en">A subtype of Parking Point located in a Garage.</rdfs:comment>
        <rdfs:comment xml:lang="en">TODO: Complete all properties</rdfs:comment>
        <rdfs:label xml:lang="en">Garage Point</rdfs:label>
    </owl:Class>
    


    <!-- https://w3id.org/transmodel/journeys#GroupOfTimingLinks -->

    <owl:Class rdf:about="https://w3id.org/transmodel/journeys#GroupOfTimingLinks">
        <rdfs:subClassOf rdf:resource="https://w3id.org/transmodel/journeys#TOREVIEWCLASSES"/>
        <rdfs:comment xml:lang="en">A set of TimingLinks grouped together according to the similarity of TimeBand which are relevant to them. There may be a GroupOfTimingLinks which covers all TimingLinks, for use when different GroupOfTimingLinks are not needed</rdfs:comment>
        <rdfs:label xml:lang="en">GroupOfTimingLink</rdfs:label>
    </owl:Class>
    


    <!-- https://w3id.org/transmodel/journeys#HeadwayInterval -->

    <owl:Class rdf:about="https://w3id.org/transmodel/journeys#HeadwayInterval">
        <rdfs:subClassOf>
            <owl:Restriction>
                <owl:onProperty rdf:resource="https://w3id.org/transmodel/journeys#maximumHeadwayInterval"/>
                <owl:maxQualifiedCardinality rdf:datatype="http://www.w3.org/2001/XMLSchema#nonNegativeInteger">1</owl:maxQualifiedCardinality>
                <owl:onDataRange rdf:resource="http://www.w3.org/2001/XMLSchema#duration"/>
            </owl:Restriction>
        </rdfs:subClassOf>
        <rdfs:subClassOf>
            <owl:Restriction>
                <owl:onProperty rdf:resource="https://w3id.org/transmodel/journeys#minimumHeadwayInterval"/>
                <owl:maxQualifiedCardinality rdf:datatype="http://www.w3.org/2001/XMLSchema#nonNegativeInteger">1</owl:maxQualifiedCardinality>
                <owl:onDataRange rdf:resource="http://www.w3.org/2001/XMLSchema#duration"/>
            </owl:Restriction>
        </rdfs:subClassOf>
        <rdfs:subClassOf>
            <owl:Restriction>
                <owl:onProperty rdf:resource="https://w3id.org/transmodel/journeys#scheduledHeadwayInterval"/>
                <owl:maxQualifiedCardinality rdf:datatype="http://www.w3.org/2001/XMLSchema#nonNegativeInteger">1</owl:maxQualifiedCardinality>
                <owl:onDataRange rdf:resource="http://www.w3.org/2001/XMLSchema#duration"/>
            </owl:Restriction>
        </rdfs:subClassOf>
        <rdfs:comment xml:lang="en">A time interval or a duration defining a headway period and characterizing Headway Journey Groups (e.g. every 10 min, every  4-6 min).</rdfs:comment>
        <rdfs:label xml:lang="en">Headway Interval</rdfs:label>
    </owl:Class>
    


    <!-- https://w3id.org/transmodel/journeys#HeadwayJourneyGroup -->

    <owl:Class rdf:about="https://w3id.org/transmodel/journeys#HeadwayJourneyGroup">
        <rdfs:subClassOf rdf:resource="https://w3id.org/transmodel/journeys#JourneyFrequencyGroup"/>
        <rdfs:subClassOf>
            <owl:Restriction>
                <owl:onProperty rdf:resource="https://w3id.org/transmodel/journeys#determinedBy"/>
                <owl:allValuesFrom rdf:resource="https://w3id.org/transmodel/journeys#HeadwayInterval"/>
            </owl:Restriction>
        </rdfs:subClassOf>
        <rdfs:comment xml:lang="en">A group of Vehicle Journeys following the same Journey Pattern having the same Headway Interval between a specified start and end time (for example, every 10 min). This is especially useful for passenger information.</rdfs:comment>
        <rdfs:comment xml:lang="en">TODO Define the TimeBand class that is describing the time band for this type of journey group, and hence can be related to this class or to its superclass.</rdfs:comment>
        <rdfs:comment xml:lang="en">TODO: Include the class Time Demand Type, which is used to specify traffic conditions or other factors which may affect vehicle run or wait times, and relate it to this class</rdfs:comment>
        <rdfs:label xml:lang="en">Headway Journey Group</rdfs:label>
    </owl:Class>
    


    <!-- https://w3id.org/transmodel/journeys#InfrastructurePoint -->

    <owl:Class rdf:about="https://w3id.org/transmodel/journeys#InfrastructurePoint">
        <rdfs:subClassOf rdf:resource="https://w3id.org/transmodel/journeys#Point"/>
        <rdfs:comment xml:lang="en">A super-type including all Points of the physical network (e.g. Railway Junction).</rdfs:comment>
        <rdfs:comment xml:lang="en">TODO: Complete with all relevant properties</rdfs:comment>
        <rdfs:label xml:lang="en">Infrastructure Point</rdfs:label>
    </owl:Class>
    


    <!-- https://w3id.org/transmodel/journeys#Journey -->

    <owl:Class rdf:about="https://w3id.org/transmodel/journeys#Journey">
        <rdfs:comment xml:lang="en">Common properties of Vehicle Journey and Special Service, e.g. their link to accounting characteristics</rdfs:comment>
        <rdfs:label xml:lang="en">Journey</rdfs:label>
    </owl:Class>
    


    <!-- https://w3id.org/transmodel/journeys#JourneyFrequencyGroup -->

    <owl:Class rdf:about="https://w3id.org/transmodel/journeys#JourneyFrequencyGroup">
        <rdfs:subClassOf>
            <owl:Restriction>
                <owl:onProperty rdf:resource="https://w3id.org/transmodel/journeys#composedOf"/>
                <owl:allValuesFrom rdf:resource="https://w3id.org/transmodel/journeys#VehicleJourney"/>
            </owl:Restriction>
        </rdfs:subClassOf>
        <rdfs:subClassOf>
            <owl:Restriction>
                <owl:onProperty rdf:resource="https://w3id.org/transmodel/journeys#firstDayOffset"/>
                <owl:allValuesFrom rdf:resource="http://www.w3.org/2001/XMLSchema#int"/>
            </owl:Restriction>
        </rdfs:subClassOf>
        <rdfs:subClassOf>
            <owl:Restriction>
                <owl:onProperty rdf:resource="https://w3id.org/transmodel/journeys#firstDepartureTime"/>
                <owl:allValuesFrom rdf:resource="http://www.w3.org/2001/XMLSchema#time"/>
            </owl:Restriction>
        </rdfs:subClassOf>
        <rdfs:subClassOf>
            <owl:Restriction>
                <owl:onProperty rdf:resource="https://w3id.org/transmodel/journeys#lastDayOffset"/>
                <owl:allValuesFrom rdf:resource="http://www.w3.org/2001/XMLSchema#int"/>
            </owl:Restriction>
        </rdfs:subClassOf>
        <rdfs:subClassOf>
            <owl:Restriction>
                <owl:onProperty rdf:resource="https://w3id.org/transmodel/journeys#lastDepartureTime"/>
                <owl:allValuesFrom rdf:resource="http://www.w3.org/2001/XMLSchema#time"/>
            </owl:Restriction>
        </rdfs:subClassOf>
        <rdfs:comment xml:lang="en">A group of Journeys defined in order to describe special behaviour like frequency based services or rhythmical services (e.g., runs all xxh10, xxh25 and xxh45). This is especially useful for passenger information).</rdfs:comment>
        <rdfs:label xml:lang="en">Journey Frequency Group</rdfs:label>
    </owl:Class>
    


    <!-- https://w3id.org/transmodel/journeys#JourneyPart -->

    <owl:Class rdf:about="https://w3id.org/transmodel/journeys#JourneyPart">
        <rdfs:subClassOf rdf:resource="https://w3id.org/transmodel/journeys#TOREVIEWCLASSES"/>
        <rdfs:comment xml:lang="en">A part of a VehicleJourney created according to a specific functional purpose, for instance in situations when Vehicle coupling or separating occurrs</rdfs:comment>
        <rdfs:label xml:lang="en">JourneyPart</rdfs:label>
    </owl:Class>
    


    <!-- https://w3id.org/transmodel/journeys#JourneyPartCouple -->

    <owl:Class rdf:about="https://w3id.org/transmodel/journeys#JourneyPartCouple">
        <rdfs:subClassOf rdf:resource="https://w3id.org/transmodel/journeys#TOREVIEWCLASSES"/>
        <rdfs:comment xml:lang="en">Two JourneyParts of different VehicleJourneys served simultaneously by a train set up by coupling their single Vehicles</rdfs:comment>
        <rdfs:label xml:lang="en">JourneyPartCouple</rdfs:label>
    </owl:Class>
    


    <!-- https://w3id.org/transmodel/journeys#JourneyPattern -->

    <owl:Class rdf:about="https://w3id.org/transmodel/journeys#JourneyPattern">
        <rdfs:subClassOf rdf:resource="https://w3id.org/transmodel/journeys#LinkSequence"/>
        <rdfs:subClassOf>
            <owl:Restriction>
                <owl:onProperty rdf:resource="https://w3id.org/transmodel/journeys#primarilyAdvertisedWith"/>
                <owl:allValuesFrom rdf:resource="https://w3id.org/transmodel/journeys#DestinationDisplay"/>
            </owl:Restriction>
        </rdfs:subClassOf>
        <rdfs:comment xml:lang="en">An ordered list of Scheduled Stop Points and Timing Points on a single Route, describing the pattern of working for public transport vehicles. A Journey Pattern may pass through the same Point more than once. The first Point of a Journey Pattern is the origin. The last Point is the destination.</rdfs:comment>
        <rdfs:label xml:lang="en">Journey Pattern</rdfs:label>
    </owl:Class>
    


    <!-- https://w3id.org/transmodel/journeys#JourneyPatternLayover -->

    <owl:Class rdf:about="https://w3id.org/transmodel/journeys#JourneyPatternLayover">
        <rdfs:subClassOf rdf:resource="https://w3id.org/transmodel/journeys#TOREVIEWCLASSES"/>
        <rdfs:comment xml:lang="en">A JourneyPatternLayover is the time allowance at the end of each journey on a specified JourneyPattern to allow for delays and for other purposes. This layover supersedes any global layover and may be superseded by a specific VehicleJourneyLayover</rdfs:comment>
        <rdfs:label xml:lang="en">JourneyPatternLayover</rdfs:label>
    </owl:Class>
    


    <!-- https://w3id.org/transmodel/journeys#JourneyPatternRunTime -->

    <owl:Class rdf:about="https://w3id.org/transmodel/journeys#JourneyPatternRunTime">
        <rdfs:subClassOf rdf:resource="https://w3id.org/transmodel/journeys#TOREVIEWCLASSES"/>
        <rdfs:comment xml:lang="en">The time taken to traverse a TimingLink in a particular JourneyPattern, for a specified TimeDemandType. If it exists, it will override the DefaultServiceJourneyRunTime and DefaultDeadRunRunTime</rdfs:comment>
        <rdfs:label xml:lang="en">JourneyPatternRunTime</rdfs:label>
    </owl:Class>
    


    <!-- https://w3id.org/transmodel/journeys#Line -->

    <owl:Class rdf:about="https://w3id.org/transmodel/journeys#Line">
        <rdfs:subClassOf>
            <owl:Restriction>
                <owl:onProperty rdf:resource="https://w3id.org/transmodel/journeys#presentedBy"/>
                <owl:allValuesFrom rdf:resource="https://w3id.org/transmodel/commons#Presentation"/>
            </owl:Restriction>
        </rdfs:subClassOf>
        <rdfs:comment xml:lang="en">A Line is a group of Routes which is generally known to the public by a similar name or number.</rdfs:comment>
        <rdfs:label xml:lang="en">Line</rdfs:label>
    </owl:Class>
    


    <!-- https://w3id.org/transmodel/journeys#Line-old -->

    <owl:Class rdf:about="https://w3id.org/transmodel/journeys#Line-old">
        <rdfs:subClassOf rdf:resource="https://w3id.org/transmodel/journeys#TOREVIEWCLASSES"/>
        <rdfs:comment xml:lang="en">A Line is a group of Route which is generally known to the public by a similar name or number.</rdfs:comment>
        <rdfs:label xml:lang="en">Line-old</rdfs:label>
    </owl:Class>
    


    <!-- https://w3id.org/transmodel/journeys#LinkSequence -->

    <owl:Class rdf:about="https://w3id.org/transmodel/journeys#LinkSequence">
        <rdfs:subClassOf>
            <owl:Restriction>
                <owl:onProperty rdf:resource="https://w3id.org/transmodel/journeys#madeUpOf"/>
                <owl:allValuesFrom rdf:resource="https://w3id.org/transmodel/journeys#PointInLinkSequence"/>
            </owl:Restriction>
        </rdfs:subClassOf>
        <rdfs:comment xml:lang="en">An ordered sequence either of POINTs or of LINKs, defining a path through the network</rdfs:comment>
        <rdfs:comment xml:lang="en">TODO: Add all the attributes that are relevant to this class</rdfs:comment>
        <rdfs:comment xml:lang="en">TODO: Analyse whether this class should be better defined in the Commons module</rdfs:comment>
        <rdfs:label xml:lang="en">Link Sequence</rdfs:label>
    </owl:Class>
    


    <!-- https://w3id.org/transmodel/journeys#MeanOfTransport -->

    <owl:Class rdf:about="https://w3id.org/transmodel/journeys#MeanOfTransport">
        <rdfs:subClassOf rdf:resource="https://w3id.org/transmodel/journeys#TOREVIEWCLASSES"/>
        <rdfs:comment xml:lang="en">Any Mode of Transport</rdfs:comment>
        <rdfs:label xml:lang="en">ModeOfTransport</rdfs:label>
    </owl:Class>
    


    <!-- https://w3id.org/transmodel/journeys#MonitoredVehicleJourney -->

    <owl:Class rdf:about="https://w3id.org/transmodel/journeys#MonitoredVehicleJourney">
        <rdfs:subClassOf rdf:resource="https://w3id.org/transmodel/journeys#VehicleJourney"/>
        <rdfs:comment xml:lang="en">A VehicleJourney that is run under real-time tracking system and so for which real-time observations and predictions and other data are available</rdfs:comment>
        <rdfs:label xml:lang="en">Monitored Vehicle Journey</rdfs:label>
    </owl:Class>
    


    <!-- https://w3id.org/transmodel/journeys#OperatingDay -->

    <owl:Class rdf:about="https://w3id.org/transmodel/journeys#OperatingDay">
        <rdfs:comment xml:lang="en">A day of public transport operation of which the characteristics are defined within in a specific ServiceCalendar. An OperatingDay may last more than 24 hours.</rdfs:comment>
        <rdfs:label xml:lang="en">Operating Day</rdfs:label>
    </owl:Class>
    


    <!-- https://w3id.org/transmodel/journeys#OperatingPeriod -->

    <owl:Class rdf:about="https://w3id.org/transmodel/journeys#OperatingPeriod">
        <rdfs:subClassOf>
            <owl:Restriction>
                <owl:onProperty rdf:resource="https://w3id.org/transmodel/journeys#endingAt"/>
                <owl:allValuesFrom rdf:resource="https://w3id.org/transmodel/journeys#OperatingDay"/>
            </owl:Restriction>
        </rdfs:subClassOf>
        <rdfs:subClassOf>
            <owl:Restriction>
                <owl:onProperty rdf:resource="https://w3id.org/transmodel/journeys#startingAt"/>
                <owl:allValuesFrom rdf:resource="https://w3id.org/transmodel/journeys#OperatingDay"/>
            </owl:Restriction>
        </rdfs:subClassOf>
        <rdfs:comment xml:lang="en">A continuous interval of time between two Operating Day which will be used to define validities</rdfs:comment>
        <rdfs:label xml:lang="en">Operating Period</rdfs:label>
    </owl:Class>
    


    <!-- https://w3id.org/transmodel/journeys#OrganisationDayType -->

    <owl:Class rdf:about="https://w3id.org/transmodel/journeys#OrganisationDayType">
        <rdfs:subClassOf rdf:resource="https://w3id.org/transmodel/journeys#DayType"/>
        <rdfs:subClassOf>
            <owl:Restriction>
                <owl:onProperty rdf:resource="https://w3id.org/transmodel/journeys#isServiceDay"/>
                <owl:allValuesFrom rdf:resource="http://www.w3.org/2001/XMLSchema#boolean"/>
            </owl:Restriction>
        </rdfs:subClassOf>
        <rdfs:comment xml:lang="en">Day Type that is defined in terms of operation or not operation of a referenced Serviced Organisation.</rdfs:comment>
        <rdfs:label xml:lang="en">Organisation Day Type</rdfs:label>
        <rdfs:label xml:lang="en">TODO: Add constraint: :forServicedOrganisation only tmorg:ServicedOrganisation</rdfs:label>
    </owl:Class>
    


    <!-- https://w3id.org/transmodel/journeys#ParkingPoint -->

    <owl:Class rdf:about="https://w3id.org/transmodel/journeys#ParkingPoint">
        <rdfs:subClassOf rdf:resource="https://w3id.org/transmodel/journeys#ReliefPoint"/>
        <rdfs:subClassOf>
            <owl:Restriction>
                <owl:onProperty rdf:resource="https://w3id.org/transmodel/journeys#endOfBlock"/>
                <owl:allValuesFrom rdf:resource="https://w3id.org/transmodel/journeys#Block"/>
            </owl:Restriction>
        </rdfs:subClassOf>
        <rdfs:subClassOf>
            <owl:Restriction>
                <owl:onProperty rdf:resource="https://w3id.org/transmodel/journeys#startOfBlock"/>
                <owl:allValuesFrom rdf:resource="https://w3id.org/transmodel/journeys#Block"/>
            </owl:Restriction>
        </rdfs:subClassOf>
        <rdfs:comment xml:lang="en">A Parking Point where Vehicles may stay unattended for a long time. A vehicle&apos;s return to the Parking Point marks the end of a Block</rdfs:comment>
        <rdfs:label xml:lang="en">Parking Point</rdfs:label>
    </owl:Class>
    


    <!-- https://w3id.org/transmodel/journeys#PassengerStopAssignment -->

    <owl:Class rdf:about="https://w3id.org/transmodel/journeys#PassengerStopAssignment">
        <rdfs:subClassOf rdf:resource="https://w3id.org/transmodel/journeys#StopAssignment"/>
        <rdfs:comment xml:lang="en">The allocation of a Scheduled Stop Point to a specific Stop Place for a Service Journey, and also possibly a Quay and Boarding Position</rdfs:comment>
        <rdfs:label xml:lang="en">Passenger Stop Assignment</rdfs:label>
    </owl:Class>
    


    <!-- https://w3id.org/transmodel/journeys#Place -->

    <owl:Class rdf:about="https://w3id.org/transmodel/journeys#Place">
        <rdfs:subClassOf rdf:resource="https://w3id.org/transmodel/journeys#TOREVIEWCLASSES"/>
        <rdfs:comment xml:lang="en">A geographic Place of any type which may be specified as the origin or destination of a Trip. A Place may be represented as a Point (dimension 0), a Road section (dimension 1) or a Zone (dimension 2)</rdfs:comment>
        <rdfs:label xml:lang="en">Place</rdfs:label>
    </owl:Class>
    


    <!-- https://w3id.org/transmodel/journeys#Point -->

    <owl:Class rdf:about="https://w3id.org/transmodel/journeys#Point">
        <rdfs:subClassOf>
            <owl:Restriction>
                <owl:onProperty rdf:resource="https://w3id.org/transmodel/journeys#aViewOf"/>
                <owl:allValuesFrom rdf:resource="https://w3id.org/transmodel/journeys#PointInLinkSequence"/>
            </owl:Restriction>
        </rdfs:subClassOf>
        <rdfs:comment xml:lang="en">A Point is a 0-dimensional Node of the Network used for the spatial description of the network. Point may be located by a Location</rdfs:comment>
        <rdfs:comment xml:lang="en">TODO: Make it in that ontology a subclass of the W3C Geo Point</rdfs:comment>
        <rdfs:comment xml:lang="en">TODO: Move this concept to Commons</rdfs:comment>
        <rdfs:label xml:lang="en">Point</rdfs:label>
    </owl:Class>
    


    <!-- https://w3id.org/transmodel/journeys#PointInJourneyPattern -->

    <owl:Class rdf:about="https://w3id.org/transmodel/journeys#PointInJourneyPattern">
        <rdfs:subClassOf rdf:resource="https://w3id.org/transmodel/journeys#PointInLinkSequence"/>
        <rdfs:subClassOf>
            <owl:Restriction>
                <owl:onProperty rdf:resource="https://w3id.org/transmodel/journeys#passesAt"/>
                <owl:allValuesFrom rdf:resource="https://w3id.org/transmodel/journeys#TimetabledPassingTime"/>
            </owl:Restriction>
        </rdfs:subClassOf>
        <rdfs:subClassOf>
            <owl:Restriction>
                <owl:onProperty rdf:resource="https://w3id.org/transmodel/journeys#prescribing"/>
                <owl:allValuesFrom rdf:resource="https://w3id.org/transmodel/journeys#DestinationDisplay"/>
            </owl:Restriction>
        </rdfs:subClassOf>
        <rdfs:comment xml:lang="en">A Scheduled Stop Point OR Timing Point in a Journey Pattern with its order in that Journey Pattern</rdfs:comment>
        <rdfs:label xml:lang="en">Point In Journey Pattern</rdfs:label>
    </owl:Class>
    


    <!-- https://w3id.org/transmodel/journeys#PointInLinkSequence -->

    <owl:Class rdf:about="https://w3id.org/transmodel/journeys#PointInLinkSequence">
        <rdfs:subClassOf>
            <owl:Restriction>
                <owl:onProperty rdf:resource="https://w3id.org/transmodel/journeys#inLinkSequence"/>
                <owl:qualifiedCardinality rdf:datatype="http://www.w3.org/2001/XMLSchema#nonNegativeInteger">1</owl:qualifiedCardinality>
                <owl:onClass rdf:resource="https://w3id.org/transmodel/journeys#LinkSequence"/>
            </owl:Restriction>
        </rdfs:subClassOf>
        <rdfs:subClassOf>
            <owl:Restriction>
                <owl:onProperty rdf:resource="https://w3id.org/transmodel/journeys#viewedAs"/>
                <owl:qualifiedCardinality rdf:datatype="http://www.w3.org/2001/XMLSchema#nonNegativeInteger">1</owl:qualifiedCardinality>
                <owl:onClass rdf:resource="https://w3id.org/transmodel/journeys#Point"/>
            </owl:Restriction>
        </rdfs:subClassOf>
        <rdfs:subClassOf>
            <owl:Restriction>
                <owl:onProperty rdf:resource="https://w3id.org/transmodel/journeys#distanceFromStart"/>
                <owl:qualifiedCardinality rdf:datatype="http://www.w3.org/2001/XMLSchema#nonNegativeInteger">1</owl:qualifiedCardinality>
                <owl:onDataRange rdf:resource="http://www.w3.org/2001/XMLSchema#float"/>
            </owl:Restriction>
        </rdfs:subClassOf>
        <rdfs:subClassOf>
            <owl:Restriction>
                <owl:onProperty rdf:resource="https://w3id.org/transmodel/journeys#order"/>
                <owl:qualifiedCardinality rdf:datatype="http://www.w3.org/2001/XMLSchema#nonNegativeInteger">1</owl:qualifiedCardinality>
                <owl:onDataRange rdf:resource="http://www.w3.org/2001/XMLSchema#nonNegativeInteger"/>
            </owl:Restriction>
        </rdfs:subClassOf>
        <rdfs:comment xml:lang="en">A point in a Link Sequence indicating its order in that particular Link Sequence</rdfs:comment>
        <rdfs:comment xml:lang="en">TODO: TransModel defines that a Point in Link Sequence is connected to a Layer, but this is not considered relevant yet</rdfs:comment>
        <rdfs:label xml:lang="en">Point In Link Sequence</rdfs:label>
    </owl:Class>
    


    <!-- https://w3id.org/transmodel/journeys#PointOnRoute -->

    <owl:Class rdf:about="https://w3id.org/transmodel/journeys#PointOnRoute">
        <rdfs:subClassOf rdf:resource="https://w3id.org/transmodel/journeys#PointInLinkSequence"/>
        <rdfs:subClassOf>
            <owl:Restriction>
                <owl:onProperty rdf:resource="https://w3id.org/transmodel/commons#in"/>
                <owl:allValuesFrom rdf:resource="https://w3id.org/transmodel/journeys#Route"/>
            </owl:Restriction>
        </rdfs:subClassOf>
        <rdfs:subClassOf>
            <owl:Restriction>
                <owl:onProperty rdf:resource="https://w3id.org/transmodel/journeys#inLinkSequence"/>
                <owl:qualifiedCardinality rdf:datatype="http://www.w3.org/2001/XMLSchema#nonNegativeInteger">1</owl:qualifiedCardinality>
                <owl:onClass rdf:resource="https://w3id.org/transmodel/journeys#Route"/>
            </owl:Restriction>
        </rdfs:subClassOf>
        <rdfs:subClassOf>
            <owl:Restriction>
                <owl:onProperty rdf:resource="https://w3id.org/transmodel/journeys#viewedAs"/>
                <owl:qualifiedCardinality rdf:datatype="http://www.w3.org/2001/XMLSchema#nonNegativeInteger">1</owl:qualifiedCardinality>
                <owl:onClass rdf:resource="https://w3id.org/transmodel/journeys#RoutePoint"/>
            </owl:Restriction>
        </rdfs:subClassOf>
        <rdfs:comment xml:lang="en">A Route Point used to define a Route with its order on that Route.</rdfs:comment>
        <rdfs:label xml:lang="en">Point on Route</rdfs:label>
    </owl:Class>
    


    <!-- https://w3id.org/transmodel/journeys#PostalAddress -->

    <owl:Class rdf:about="https://w3id.org/transmodel/journeys#PostalAddress">
        <rdfs:subClassOf rdf:resource="https://w3id.org/transmodel/journeys#Address"/>
        <rdfs:comment xml:lang="en">A specification of Address refining it by using the attributes used for conventional identification for mail. Comprises variously a building identifier, Streeet name, Post Code and other descriptions.</rdfs:comment>
        <rdfs:comment xml:lang="en">PostalAddress</rdfs:comment>
    </owl:Class>
    


    <!-- https://w3id.org/transmodel/journeys#PropertyOfDay -->

    <owl:Class rdf:about="https://w3id.org/transmodel/journeys#PropertyOfDay">
        <rdfs:subClassOf>
            <owl:Restriction>
                <owl:onProperty rdf:resource="https://w3id.org/transmodel/journeys#definedAs"/>
                <owl:allValuesFrom>
                    <owl:Class>
                        <owl:intersectionOf rdf:parseType="Collection">
                            <rdf:Description rdf:about="http://www.w3.org/2004/02/skos/core#Concept"/>
                            <owl:Restriction>
                                <owl:onProperty rdf:resource="http://www.w3.org/2004/02/skos/core#inScheme"/>
                                <owl:hasValue rdf:resource="https://w3id.org/transmodel/kos/journeys/day-type"/>
                            </owl:Restriction>
                        </owl:intersectionOf>
                    </owl:Class>
                </owl:allValuesFrom>
            </owl:Restriction>
        </rdfs:subClassOf>
        <rdfs:comment xml:lang="en">A property which a day may possess, such as school holiday, weekday, summer, winter, etc.</rdfs:comment>
        <rdfs:label xml:lang="en">Property Of Day</rdfs:label>
    </owl:Class>
    


    <!-- https://w3id.org/transmodel/journeys#RailwayJunction -->

    <owl:Class rdf:about="https://w3id.org/transmodel/journeys#RailwayJunction">
        <rdfs:subClassOf rdf:resource="https://w3id.org/transmodel/journeys#InfrastructurePoint"/>
        <rdfs:comment xml:lang="en">TODO: Complete with all relevant properties</rdfs:comment>
        <rdfs:label xml:lang="en">Railway Junction</rdfs:label>
    </owl:Class>
    


    <!-- https://w3id.org/transmodel/journeys#ReliefPoint -->

    <owl:Class rdf:about="https://w3id.org/transmodel/journeys#ReliefPoint">
        <rdfs:subClassOf rdf:resource="https://w3id.org/transmodel/journeys#TimingPoint"/>
        <rdfs:comment xml:lang="en">A Timing Point where a relief is possible, i.e. a driver may take on or hand over a vehicle. The vehicle may sometimes be left unattended.</rdfs:comment>
        <rdfs:comment xml:lang="en">TODO: Complete all properties</rdfs:comment>
        <rdfs:label xml:lang="en">Relief Point</rdfs:label>
    </owl:Class>
    


    <!-- https://w3id.org/transmodel/journeys#RhythmicalJourneyGroup -->

    <owl:Class rdf:about="https://w3id.org/transmodel/journeys#RhythmicalJourneyGroup">
        <rdfs:subClassOf rdf:resource="https://w3id.org/transmodel/journeys#JourneyFrequencyGroup"/>
        <rdfs:subClassOf>
            <owl:Restriction>
                <owl:onProperty rdf:resource="https://w3id.org/transmodel/journeys#defines"/>
                <owl:allValuesFrom rdf:resource="https://w3id.org/transmodel/journeys#TemplateVehicleJourney"/>
            </owl:Restriction>
        </rdfs:subClassOf>
        <rdfs:comment xml:lang="en">A group of Vehicle Journeys following  the same Journey Pattern having the same &quot;rhythm&quot; every hour (for example runs at xxh10, xxh25 and xxh45... ) between a specified start and end time.</rdfs:comment>
        <rdfs:comment xml:lang="en">TODO Define the TimeBand class that is describing the time band for this type of journey group, and hence can be related to this class or to its superclass.</rdfs:comment>
        <rdfs:label xml:lang="en">Rhythmical Journey Group</rdfs:label>
    </owl:Class>
    


    <!-- https://w3id.org/transmodel/journeys#RoadAddress -->

    <owl:Class rdf:about="https://w3id.org/transmodel/journeys#RoadAddress">
        <rdfs:subClassOf rdf:resource="https://w3id.org/transmodel/journeys#Address"/>
        <rdfs:comment xml:lang="en">Specialisation of Address refining it by using the characteristics such as road number and mname use for conventional inidentification of along a road</rdfs:comment>
        <rdfs:label xml:lang="en">RoadAddress</rdfs:label>
    </owl:Class>
    


    <!-- https://w3id.org/transmodel/journeys#RoadJunction -->

    <owl:Class rdf:about="https://w3id.org/transmodel/journeys#RoadJunction">
        <rdfs:subClassOf rdf:resource="https://w3id.org/transmodel/journeys#InfrastructurePoint"/>
        <rdfs:comment xml:lang="en">TODO: Complete with all relevant properties</rdfs:comment>
        <rdfs:label xml:lang="en">Road Junction</rdfs:label>
    </owl:Class>
    


    <!-- https://w3id.org/transmodel/journeys#Route -->

    <owl:Class rdf:about="https://w3id.org/transmodel/journeys#Route">
        <rdfs:subClassOf rdf:resource="https://w3id.org/transmodel/journeys#LinkSequence"/>
        <rdfs:comment xml:lang="en">A Route is and ordered list of located Points defining one single path through the road (or rail) network.</rdfs:comment>
        <rdfs:label xml:lang="en">Route</rdfs:label>
    </owl:Class>
    


    <!-- https://w3id.org/transmodel/journeys#RoutePoint -->

    <owl:Class rdf:about="https://w3id.org/transmodel/journeys#RoutePoint">
        <rdfs:subClassOf rdf:resource="https://w3id.org/transmodel/journeys#Point"/>
        <rdfs:subClassOf>
            <owl:Restriction>
                <owl:onProperty rdf:resource="https://w3id.org/transmodel/commons#borderCrossing"/>
                <owl:maxQualifiedCardinality rdf:datatype="http://www.w3.org/2001/XMLSchema#nonNegativeInteger">1</owl:maxQualifiedCardinality>
                <owl:onDataRange rdf:resource="http://www.w3.org/2001/XMLSchema#boolean"/>
            </owl:Restriction>
        </rdfs:subClassOf>
        <rdfs:subClassOf>
            <owl:Restriction>
                <owl:onProperty rdf:resource="https://w3id.org/transmodel/journeys#viaFlag"/>
                <owl:maxQualifiedCardinality rdf:datatype="http://www.w3.org/2001/XMLSchema#nonNegativeInteger">1</owl:maxQualifiedCardinality>
                <owl:onDataRange rdf:resource="http://www.w3.org/2001/XMLSchema#boolean"/>
            </owl:Restriction>
        </rdfs:subClassOf>
        <rdfs:comment xml:lang="en">A Point used to define the shape of a Route through the network.</rdfs:comment>
        <rdfs:label xml:lang="en">Route Point</rdfs:label>
    </owl:Class>
    


    <!-- https://w3id.org/transmodel/journeys#ScheduledStopPoint -->

    <owl:Class rdf:about="https://w3id.org/transmodel/journeys#ScheduledStopPoint">
        <rdfs:subClassOf rdf:resource="https://w3id.org/transmodel/journeys#Point"/>
        <rdfs:subClassOf>
            <owl:Restriction>
                <owl:onProperty rdf:resource="https://w3id.org/transmodel/journeys#aViewOf"/>
                <owl:allValuesFrom rdf:resource="https://w3id.org/transmodel/journeys#StopPointInJourneyPattern"/>
            </owl:Restriction>
        </rdfs:subClassOf>
        <rdfs:comment xml:lang="en">A Scheduled Stop Point is a Point where a Passenger can board or alight from a Vehicle.</rdfs:comment>
        <rdfs:label xml:lang="en">Scheduled Stop Point</rdfs:label>
    </owl:Class>
    


    <!-- https://w3id.org/transmodel/journeys#ServiceCalendar -->

    <owl:Class rdf:about="https://w3id.org/transmodel/journeys#ServiceCalendar">
        <rdfs:subClassOf rdf:resource="https://w3id.org/transmodel/journeys#TOREVIEWCLASSES"/>
        <rdfs:label xml:lang="en">ServiceCalendar</rdfs:label>
    </owl:Class>
    


    <!-- https://w3id.org/transmodel/journeys#ServiceJourney -->

    <owl:Class rdf:about="https://w3id.org/transmodel/journeys#ServiceJourney">
        <rdfs:subClassOf rdf:resource="https://w3id.org/transmodel/journeys#VehicleJourney"/>
        <rdfs:subClassOf>
            <owl:Restriction>
                <owl:onProperty rdf:resource="https://w3id.org/transmodel/journeys#directionType_old"/>
                <owl:allValuesFrom>
                    <owl:Class>
                        <owl:intersectionOf rdf:parseType="Collection">
                            <rdf:Description rdf:about="http://www.w3.org/2004/02/skos/core#Concept"/>
                            <owl:Restriction>
                                <owl:onProperty rdf:resource="http://www.w3.org/2004/02/skos/core#inScheme"/>
                                <owl:hasValue rdf:resource="https://w3id.org/transmodel/kos/journeys/direction-type"/>
                            </owl:Restriction>
                        </owl:intersectionOf>
                    </owl:Class>
                </owl:allValuesFrom>
            </owl:Restriction>
        </rdfs:subClassOf>
        <rdfs:subClassOf>
            <owl:Restriction>
                <owl:onProperty rdf:resource="https://w3id.org/transmodel/journeys#madeUsing"/>
                <owl:allValuesFrom rdf:resource="https://w3id.org/transmodel/facilities#ServiceFacilitySet"/>
            </owl:Restriction>
        </rdfs:subClassOf>
        <rdfs:comment xml:lang="en">A Service Journey is a passenger-carrying Vehicle Journey for one specified Day Type. The pattern of working is in principle defined by a Service Journey Pattern.</rdfs:comment>
        <rdfs:comment xml:lang="en">TODO: Add object properties to relate the Service Journey to other classes such as Service Journey Interchange, PT Ride Leg, Check constraint and flexible Service properties, and Vehicle Type</rdfs:comment>
        <rdfs:comment xml:lang="en">TODO: Add properties for Dynamic, Print and ServiceAlteration (as per the TransModel model)</rdfs:comment>
        <rdfs:label xml:lang="en">Service Journey</rdfs:label>
    </owl:Class>
    


    <!-- https://w3id.org/transmodel/journeys#ServiceJourneyPattern -->

    <owl:Class rdf:about="https://w3id.org/transmodel/journeys#ServiceJourneyPattern">
        <rdfs:subClassOf rdf:resource="https://w3id.org/transmodel/journeys#JourneyPattern"/>
        <rdfs:comment xml:lang="en">The Journey Pattern for (a Passenger carrying) Service Journeys</rdfs:comment>
        <rdfs:label xml:lang="en">Service Journey Pattern</rdfs:label>
    </owl:Class>
    


    <!-- https://w3id.org/transmodel/journeys#StopArea -->

    <owl:Class rdf:about="https://w3id.org/transmodel/journeys#StopArea">
        <rdfs:subClassOf rdf:resource="https://w3id.org/transmodel/journeys#TOREVIEWCLASSES"/>
        <rdfs:comment xml:lang="en">A group of Scheduled Stop Points close to each other</rdfs:comment>
        <rdfs:label xml:lang="en">Stop Area</rdfs:label>
    </owl:Class>
    


    <!-- https://w3id.org/transmodel/journeys#StopAssignment -->

    <owl:Class rdf:about="https://w3id.org/transmodel/journeys#StopAssignment">
        <rdfs:subClassOf>
            <owl:Restriction>
                <owl:onProperty rdf:resource="https://w3id.org/transmodel/journeys#for"/>
                <owl:allValuesFrom>
                    <owl:Class>
                        <owl:unionOf rdf:parseType="Collection">
                            <rdf:Description rdf:about="https://w3id.org/transmodel/facilities#BoardingPosition"/>
                            <rdf:Description rdf:about="https://w3id.org/transmodel/facilities#Quay"/>
                            <rdf:Description rdf:about="https://w3id.org/transmodel/facilities#StopPlace"/>
                            <rdf:Description rdf:about="https://w3id.org/transmodel/journeys#ScheduledStopPoint"/>
                        </owl:unionOf>
                    </owl:Class>
                </owl:allValuesFrom>
            </owl:Restriction>
        </rdfs:subClassOf>
        <rdfs:comment xml:lang="en">TODO: Add more subclasses of this class, such as TrainStopAssignment, FlexibleStopAssignment, VehicleTypeStopAssignment or NavigationPathAssignment</rdfs:comment>
        <rdfs:comment xml:lang="en">The allocation of a Scheduled Stop Point (i.e. a Scheduled Stop Point of a Service Pattern or Journey Pattner) to a specific Stop Place, for either a Service Journey or Vehicle Service.</rdfs:comment>
        <rdfs:label xml:lang="en">Stop Assignment</rdfs:label>
    </owl:Class>
    


    <!-- https://w3id.org/transmodel/journeys#StopPointInJourneyPattern -->

    <owl:Class rdf:about="https://w3id.org/transmodel/journeys#StopPointInJourneyPattern">
        <rdfs:subClassOf rdf:resource="https://w3id.org/transmodel/journeys#PointInJourneyPattern"/>
        <rdfs:subClassOf>
            <owl:Restriction>
                <owl:onProperty rdf:resource="https://w3id.org/transmodel/journeys#inLinkSequence"/>
                <owl:qualifiedCardinality rdf:datatype="http://www.w3.org/2001/XMLSchema#nonNegativeInteger">1</owl:qualifiedCardinality>
                <owl:onClass rdf:resource="https://w3id.org/transmodel/journeys#JourneyPattern"/>
            </owl:Restriction>
        </rdfs:subClassOf>
        <rdfs:subClassOf>
            <owl:Restriction>
                <owl:onProperty rdf:resource="https://w3id.org/transmodel/journeys#viewedAs"/>
                <owl:qualifiedCardinality rdf:datatype="http://www.w3.org/2001/XMLSchema#nonNegativeInteger">1</owl:qualifiedCardinality>
                <owl:onClass rdf:resource="https://w3id.org/transmodel/journeys#ScheduledStopPoint"/>
            </owl:Restriction>
        </rdfs:subClassOf>
        <rdfs:subClassOf>
            <owl:Restriction>
                <owl:onProperty rdf:resource="https://w3id.org/transmodel/journeys#stopUse"/>
                <owl:maxQualifiedCardinality rdf:datatype="http://www.w3.org/2001/XMLSchema#nonNegativeInteger">1</owl:maxQualifiedCardinality>
                <owl:onClass>
                    <owl:Class>
                        <owl:intersectionOf rdf:parseType="Collection">
                            <rdf:Description rdf:about="http://www.w3.org/2004/02/skos/core#Concept"/>
                            <owl:Restriction>
                                <owl:onProperty rdf:resource="http://www.w3.org/2004/02/skos/core#inScheme"/>
                                <owl:hasValue rdf:resource="https://w3id.org/transmodel/kos/journeys/stop-use-type"/>
                            </owl:Restriction>
                        </owl:intersectionOf>
                    </owl:Class>
                </owl:onClass>
            </owl:Restriction>
        </rdfs:subClassOf>
        <rdfs:subClassOf>
            <owl:Restriction>
                <owl:onProperty rdf:resource="https://w3id.org/transmodel/journeys#changeOfDestinationDisplay"/>
                <owl:maxQualifiedCardinality rdf:datatype="http://www.w3.org/2001/XMLSchema#nonNegativeInteger">1</owl:maxQualifiedCardinality>
                <owl:onDataRange rdf:resource="http://www.w3.org/2001/XMLSchema#boolean"/>
            </owl:Restriction>
        </rdfs:subClassOf>
        <rdfs:subClassOf>
            <owl:Restriction>
                <owl:onProperty rdf:resource="https://w3id.org/transmodel/journeys#changeOfServiceRequirements"/>
                <owl:maxQualifiedCardinality rdf:datatype="http://www.w3.org/2001/XMLSchema#nonNegativeInteger">1</owl:maxQualifiedCardinality>
                <owl:onDataRange rdf:resource="http://www.w3.org/2001/XMLSchema#boolean"/>
            </owl:Restriction>
        </rdfs:subClassOf>
        <rdfs:subClassOf>
            <owl:Restriction>
                <owl:onProperty rdf:resource="https://w3id.org/transmodel/journeys#forAlighting"/>
                <owl:maxQualifiedCardinality rdf:datatype="http://www.w3.org/2001/XMLSchema#nonNegativeInteger">1</owl:maxQualifiedCardinality>
                <owl:onDataRange rdf:resource="http://www.w3.org/2001/XMLSchema#boolean"/>
            </owl:Restriction>
        </rdfs:subClassOf>
        <rdfs:subClassOf>
            <owl:Restriction>
                <owl:onProperty rdf:resource="https://w3id.org/transmodel/journeys#forBoarding"/>
                <owl:maxQualifiedCardinality rdf:datatype="http://www.w3.org/2001/XMLSchema#nonNegativeInteger">1</owl:maxQualifiedCardinality>
                <owl:onDataRange rdf:resource="http://www.w3.org/2001/XMLSchema#boolean"/>
            </owl:Restriction>
        </rdfs:subClassOf>
        <rdfs:subClassOf>
            <owl:Restriction>
                <owl:onProperty rdf:resource="https://w3id.org/transmodel/journeys#isFlexible"/>
                <owl:maxQualifiedCardinality rdf:datatype="http://www.w3.org/2001/XMLSchema#nonNegativeInteger">1</owl:maxQualifiedCardinality>
                <owl:onDataRange rdf:resource="http://www.w3.org/2001/XMLSchema#boolean"/>
            </owl:Restriction>
        </rdfs:subClassOf>
        <rdfs:subClassOf>
            <owl:Restriction>
                <owl:onProperty rdf:resource="https://w3id.org/transmodel/journeys#requestStop"/>
                <owl:maxQualifiedCardinality rdf:datatype="http://www.w3.org/2001/XMLSchema#nonNegativeInteger">1</owl:maxQualifiedCardinality>
                <owl:onDataRange rdf:resource="http://www.w3.org/2001/XMLSchema#boolean"/>
            </owl:Restriction>
        </rdfs:subClassOf>
        <rdfs:comment xml:lang="en">A Point in Journey Pattern that is a Scheduled Stop Point</rdfs:comment>
        <rdfs:comment xml:lang="en">TODO: determine whether we need to add a property isFlexible in order to describe whether the stop has some flexilbility in the type of drop-off/pick-up, etc.</rdfs:comment>
        <rdfs:label xml:lang="en">Stop Point In Journey Pattern</rdfs:label>
    </owl:Class>
    


    <!-- https://w3id.org/transmodel/journeys#TOREVIEWCLASSES -->

    <owl:Class rdf:about="https://w3id.org/transmodel/journeys#TOREVIEWCLASSES"/>
    


    <!-- https://w3id.org/transmodel/journeys#TemplateServiceJourney -->

    <owl:Class rdf:about="https://w3id.org/transmodel/journeys#TemplateServiceJourney">
        <rdfs:subClassOf rdf:resource="https://w3id.org/transmodel/journeys#ServiceJourney"/>
        <rdfs:subClassOf rdf:resource="https://w3id.org/transmodel/journeys#TemplateVehicleJourney"/>
        <rdfs:comment xml:lang="en">A passenger-carrying Template Vehicle Journey. It may represent multiple journeys.</rdfs:comment>
        <rdfs:label xml:lang="en">Template Service Journey</rdfs:label>
    </owl:Class>
    


    <!-- https://w3id.org/transmodel/journeys#TemplateVehicleJourney -->

    <owl:Class rdf:about="https://w3id.org/transmodel/journeys#TemplateVehicleJourney">
        <rdfs:subClassOf rdf:resource="https://w3id.org/transmodel/journeys#VehicleJourney"/>
        <rdfs:subClassOf>
            <owl:Restriction>
                <owl:onProperty rdf:resource="https://w3id.org/transmodel/journeys#isDefinedBy"/>
                <owl:allValuesFrom rdf:resource="https://w3id.org/transmodel/journeys#RhythmicalJourneyGroup"/>
            </owl:Restriction>
        </rdfs:subClassOf>
        <rdfs:comment xml:lang="en">A repeating Vehicle Journey for which a frequency has been specified, either as a Headway Journey Group (e.g. every 20 minutes) or a Rhythmical Journey Group (e.g. at 15, 27 and 40 minutes past the hour). It may thus represent multiple journeys.</rdfs:comment>
        <rdfs:label xml:lang="en">Template Vehicle Journey</rdfs:label>
    </owl:Class>
    


    <!-- https://w3id.org/transmodel/journeys#TimeBand -->

    <owl:Class rdf:about="https://w3id.org/transmodel/journeys#TimeBand">
        <rdfs:subClassOf rdf:resource="https://w3id.org/transmodel/journeys#TOREVIEWCLASSES"/>
        <rdfs:comment xml:lang="en">A period in a day, significant for some aspect of public transport, e.g. similar traffic conditions or fare category</rdfs:comment>
        <rdfs:label xml:lang="en">TimeBand</rdfs:label>
    </owl:Class>
    


    <!-- https://w3id.org/transmodel/journeys#TimeDemandType -->

    <owl:Class rdf:about="https://w3id.org/transmodel/journeys#TimeDemandType">
        <rdfs:subClassOf rdf:resource="https://w3id.org/transmodel/journeys#TOREVIEWCLASSES"/>
        <rdfs:comment xml:lang="en">An indicator of traffic conditions or other factors which may affect Vehicle Run or Wait times. It may be entered directly by the scheduler or defined by the use of TimeBands.</rdfs:comment>
        <rdfs:label xml:lang="en">TimeDemandType</rdfs:label>
    </owl:Class>
    


    <!-- https://w3id.org/transmodel/journeys#TimetabledPassingTime -->

    <owl:Class rdf:about="https://w3id.org/transmodel/journeys#TimetabledPassingTime">
        <rdfs:subClassOf>
            <owl:Restriction>
                <owl:onProperty rdf:resource="https://w3id.org/transmodel/journeys#passesAt"/>
                <owl:allValuesFrom rdf:resource="https://w3id.org/transmodel/journeys#PointInJourneyPattern"/>
            </owl:Restriction>
        </rdfs:subClassOf>
        <rdfs:subClassOf>
            <owl:Restriction>
                <owl:onProperty rdf:resource="https://w3id.org/transmodel/journeys#arrivalDayOffset"/>
                <owl:allValuesFrom rdf:resource="http://www.w3.org/2001/XMLSchema#time"/>
            </owl:Restriction>
        </rdfs:subClassOf>
        <rdfs:subClassOf>
            <owl:Restriction>
                <owl:onProperty rdf:resource="https://w3id.org/transmodel/journeys#arrivalTime"/>
                <owl:allValuesFrom rdf:resource="http://www.w3.org/2001/XMLSchema#time"/>
            </owl:Restriction>
        </rdfs:subClassOf>
        <rdfs:subClassOf>
            <owl:Restriction>
                <owl:onProperty rdf:resource="https://w3id.org/transmodel/journeys#departureDayOffset"/>
                <owl:allValuesFrom rdf:resource="http://www.w3.org/2001/XMLSchema#time"/>
            </owl:Restriction>
        </rdfs:subClassOf>
        <rdfs:subClassOf>
            <owl:Restriction>
                <owl:onProperty rdf:resource="https://w3id.org/transmodel/journeys#departureTime"/>
                <owl:allValuesFrom rdf:resource="http://www.w3.org/2001/XMLSchema#time"/>
            </owl:Restriction>
        </rdfs:subClassOf>
        <rdfs:comment xml:lang="en">Long-term planned time data concerning public transport Vehicles passing a particular POINT IN JOURNEY PATTERN on a specified VEHICLE JOURNEY for a certain DAY TYPE.</rdfs:comment>
        <rdfs:label xml:lang="en">Timetabled Passing Time</rdfs:label>
    </owl:Class>
    


    <!-- https://w3id.org/transmodel/journeys#TimetabledVehicleJourney -->

    <owl:Class rdf:about="https://w3id.org/transmodel/journeys#TimetabledVehicleJourney">
        <rdfs:subClassOf rdf:resource="https://w3id.org/transmodel/journeys#VehicleJourney"/>
        <rdfs:comment xml:lang="en">The planned movement of a Public Transport Vehicle on a Day Type from the start point to the end point of a Journey Pattern on a specified Route.</rdfs:comment>
        <rdfs:label xml:lang="en">Timetabled Vehicle Journey</rdfs:label>
    </owl:Class>
    


    <!-- https://w3id.org/transmodel/journeys#TimingLink -->

    <owl:Class rdf:about="https://w3id.org/transmodel/journeys#TimingLink">
        <rdfs:subClassOf rdf:resource="https://w3id.org/transmodel/journeys#TOREVIEWCLASSES"/>
        <rdfs:comment xml:lang="en">A TimingLink is an ordered pair of TimingPoint for which run times
may be recorded.</rdfs:comment>
        <rdfs:label xml:lang="en">TimingLink</rdfs:label>
    </owl:Class>
    


    <!-- https://w3id.org/transmodel/journeys#TimingLinkInJourneyPattern -->

    <owl:Class rdf:about="https://w3id.org/transmodel/journeys#TimingLinkInJourneyPattern">
        <rdfs:subClassOf rdf:resource="https://w3id.org/transmodel/journeys#TOREVIEWCLASSES"/>
        <rdfs:comment xml:lang="en">A TimingLinkInJourneyPattern is the position of a TimingLink in a
JourneyPattern. This entity is needed if a TimingLink is repeated
in the same JourneyPattern, and separate information is to be stored
about each iteration of the TimingLink</rdfs:comment>
        <rdfs:label xml:lang="en">TimingLinkInJourneyPattern</rdfs:label>
    </owl:Class>
    


    <!-- https://w3id.org/transmodel/journeys#TimingPoint -->

    <owl:Class rdf:about="https://w3id.org/transmodel/journeys#TimingPoint">
        <rdfs:subClassOf rdf:resource="https://w3id.org/transmodel/journeys#Point"/>
        <rdfs:subClassOf>
            <owl:Restriction>
                <owl:onProperty rdf:resource="https://w3id.org/transmodel/journeys#aViewOf"/>
                <owl:allValuesFrom rdf:resource="https://w3id.org/transmodel/journeys#TimingPointInJourneyPattern"/>
            </owl:Restriction>
        </rdfs:subClassOf>
        <rdfs:comment xml:lang="en">A Timing Point is a Point against which the timing information necessary to build schedules may be recorded.

It&apos;s the same as Timing Point In Journey Pattern</rdfs:comment>
        <rdfs:label xml:lang="en">Timing Point</rdfs:label>
    </owl:Class>
    


    <!-- https://w3id.org/transmodel/journeys#TimingPointInJourneyPattern -->

    <owl:Class rdf:about="https://w3id.org/transmodel/journeys#TimingPointInJourneyPattern">
        <rdfs:subClassOf rdf:resource="https://w3id.org/transmodel/journeys#PointInJourneyPattern"/>
        <rdfs:subClassOf>
            <owl:Restriction>
                <owl:onProperty rdf:resource="https://w3id.org/transmodel/journeys#viewedAs"/>
                <owl:qualifiedCardinality rdf:datatype="http://www.w3.org/2001/XMLSchema#nonNegativeInteger">1</owl:qualifiedCardinality>
                <owl:onClass rdf:resource="https://w3id.org/transmodel/journeys#TimingPoint"/>
            </owl:Restriction>
        </rdfs:subClassOf>
        <rdfs:subClassOf>
            <owl:Restriction>
                <owl:onProperty rdf:resource="https://w3id.org/transmodel/journeys#isWaitPoint"/>
                <owl:allValuesFrom rdf:resource="http://www.w3.org/2001/XMLSchema#boolean"/>
            </owl:Restriction>
        </rdfs:subClassOf>
        <rdfs:comment xml:lang="en">A Point in a Journey Pattern which is a Timing Point</rdfs:comment>
        <rdfs:label xml:lang="en">Timing Point In Journey Pattern</rdfs:label>
    </owl:Class>
    


    <!-- https://w3id.org/transmodel/journeys#TopographicPlace -->

    <owl:Class rdf:about="https://w3id.org/transmodel/journeys#TopographicPlace">
        <rdfs:subClassOf rdf:resource="https://w3id.org/transmodel/journeys#Place"/>
        <rdfs:comment xml:lang="en">A type of Place providing the topographical context when searching for or presenting travel information, for example as the origin or destination of a trip. It may be of any size (e.g. County, City, Town, Village) and of different specificity (e.g. Greater London, London, West End, Westimenster, St James)</rdfs:comment>
        <rdfs:label xml:lang="en">TopographicPlace</rdfs:label>
    </owl:Class>
    


    <!-- https://w3id.org/transmodel/journeys#TrafficControlPoint -->

    <owl:Class rdf:about="https://w3id.org/transmodel/journeys#TrafficControlPoint">
        <rdfs:subClassOf rdf:resource="https://w3id.org/transmodel/journeys#Point"/>
        <rdfs:comment xml:lang="en">A Point where the traffic flow can be influenced. Examples are: traffic lights (lanterns), barriers.</rdfs:comment>
        <rdfs:comment xml:lang="en">TODO: Complete with all relevant properties</rdfs:comment>
        <rdfs:label xml:lang="en">Traffic Control Point</rdfs:label>
    </owl:Class>
    


    <!-- https://w3id.org/transmodel/journeys#Trip -->

    <owl:Class rdf:about="https://w3id.org/transmodel/journeys#Trip">
        <rdfs:subClassOf rdf:resource="https://w3id.org/transmodel/journeys#TOREVIEWCLASSES"/>
        <rdfs:comment xml:lang="en">According to the definition of GTFS for Trip the VehicleJourney&apos;s Transmodel definition would fit better</rdfs:comment>
        <rdfs:comment xml:lang="en">In Transmodel is the physical spatial possibility for a passenger to travel from a Place (located Point) origin of the Trip to another place (located Point) destination of the Trip.</rdfs:comment>
        <rdfs:label xml:lang="en">Trip</rdfs:label>
    </owl:Class>
    


    <!-- https://w3id.org/transmodel/journeys#Vehicle -->

    <owl:Class rdf:about="https://w3id.org/transmodel/journeys#Vehicle">
        <rdfs:subClassOf rdf:resource="https://w3id.org/transmodel/journeys#TOREVIEWCLASSES"/>
        <rdfs:comment xml:lang="en">A PublicTransportVehicle used for carrying Passengers</rdfs:comment>
        <rdfs:label xml:lang="en">Vehicle</rdfs:label>
    </owl:Class>
    


    <!-- https://w3id.org/transmodel/journeys#VehicleJourney -->

    <owl:Class rdf:about="https://w3id.org/transmodel/journeys#VehicleJourney">
        <rdfs:subClassOf rdf:resource="https://w3id.org/transmodel/journeys#Journey"/>
        <rdfs:subClassOf>
            <owl:Restriction>
                <owl:onProperty rdf:resource="https://w3id.org/transmodel/commons#in"/>
                <owl:allValuesFrom rdf:resource="https://w3id.org/transmodel/journeys#Block"/>
            </owl:Restriction>
        </rdfs:subClassOf>
        <rdfs:subClassOf>
            <owl:Restriction>
                <owl:onProperty rdf:resource="https://w3id.org/transmodel/journeys#passesAt"/>
                <owl:allValuesFrom rdf:resource="https://w3id.org/transmodel/journeys#TimetabledPassingTime"/>
            </owl:Restriction>
        </rdfs:subClassOf>
        <rdfs:subClassOf>
            <owl:Restriction>
                <owl:onProperty rdf:resource="https://w3id.org/transmodel/journeys#runsOn"/>
                <owl:allValuesFrom rdf:resource="https://w3id.org/transmodel/journeys#JourneyFrequencyGroup"/>
            </owl:Restriction>
        </rdfs:subClassOf>
        <rdfs:comment xml:lang="en">A Vehicle Journey is the journey made by the Vehicle.

A Service Journey is made of Vehicle Journeys

Within VehicleJourney there are several types:
- Timetabled Vehicle Journey in a general timetable that will run on a specific time on a Day Type throughout the period of applicability of the schedule.
- Dated Vehicle Journey, a specific Vehicle Journey that runs on a spcific calendar date;
- Monitored Vehicle Journey, a Vehicle Journey run under real-time tracking system and so for which real-time observations and predictions and other data are available.
- Dead Run, a Vehicle Journey without service</rdfs:comment>
        <rdfs:label xml:lang="en">Vehicle Journey</rdfs:label>
    </owl:Class>
    


    <!-- https://w3id.org/transmodel/journeys#VehicleJourneyLayover -->

    <owl:Class rdf:about="https://w3id.org/transmodel/journeys#VehicleJourneyLayover">
        <rdfs:subClassOf rdf:resource="https://w3id.org/transmodel/journeys#TOREVIEWCLASSES"/>
        <rdfs:label xml:lang="en">VehicleJourneyLayover</rdfs:label>
    </owl:Class>
    


    <!-- https://w3id.org/transmodel/journeys#VehicleJourneyRunTime -->

    <owl:Class rdf:about="https://w3id.org/transmodel/journeys#VehicleJourneyRunTime">
        <rdfs:subClassOf rdf:resource="https://w3id.org/transmodel/journeys#TOREVIEWCLASSES"/>
        <rdfs:comment xml:lang="en">The time taken to traverse a specified TimingLinkInJourneyPattern on a specified VehicleJourney. This gives the most detailed control over times and overrides the DefaultServiceJourneyRunTime and JourneyPatternRunTime and the DefaultDeadRunRunTime</rdfs:comment>
        <rdfs:label xml:lang="en">VehicleJourneyRunTime</rdfs:label>
    </owl:Class>
    


    <!-- https://w3id.org/transmodel/journeys#VehicleMode -->

    <owl:Class rdf:about="https://w3id.org/transmodel/journeys#VehicleMode">
        <rdfs:comment xml:lang="en">A characterisation of the public transport operation according to the means of transport (bus, tram, metro, train, ferry, ship).</rdfs:comment>
        <rdfs:label xml:lang="en">Vehicle Mode</rdfs:label>
    </owl:Class>
    


    <!-- https://w3id.org/transmodel/journeys#WireJunction -->

    <owl:Class rdf:about="https://w3id.org/transmodel/journeys#WireJunction">
        <rdfs:subClassOf rdf:resource="https://w3id.org/transmodel/journeys#InfrastructurePoint"/>
        <rdfs:comment xml:lang="en">TODO: Complete with all relevant properties</rdfs:comment>
        <rdfs:label xml:lang="en">Wire Junction</rdfs:label>
    </owl:Class>
    


    <!-- https://w3id.org/transmodel/organisations#Operator -->

    <owl:Class rdf:about="https://w3id.org/transmodel/organisations#Operator">
        <rdfs:comment xml:lang="en">A company providing Public Transport Services. In GTFS, this is represented as a TransitAgency</rdfs:comment>
        <rdfs:comment xml:lang="en">The class comes from tm-organisations.owl</rdfs:comment>
        <rdfs:label xml:lang="es">Operator</rdfs:label>
    </owl:Class>
    


    <!-- 
    ///////////////////////////////////////////////////////////////////////////////////////
    //
    // Individuals
    //
    ///////////////////////////////////////////////////////////////////////////////////////
     -->

    


    <!-- https://w3id.org/transmodel/journeys#BothDirections -->

    <owl:NamedIndividual rdf:about="https://w3id.org/transmodel/journeys#BothDirections">
        <rdf:type rdf:resource="https://w3id.org/transmodel/journeys#AllowedLineDirections"/>
        <rdfs:label xml:lang="en">BothDirections</rdfs:label>
    </owl:NamedIndividual>
    


    <!-- https://w3id.org/transmodel/journeys#Bus -->

    <owl:NamedIndividual rdf:about="https://w3id.org/transmodel/journeys#Bus">
        <rdf:type rdf:resource="https://w3id.org/transmodel/journeys#MeanOfTransport"/>
        <rdfs:label xml:lang="en">Bus</rdfs:label>
    </owl:NamedIndividual>
    


    <!-- https://w3id.org/transmodel/journeys#CableCar -->

    <owl:NamedIndividual rdf:about="https://w3id.org/transmodel/journeys#CableCar">
        <rdf:type rdf:resource="https://w3id.org/transmodel/journeys#MeanOfTransport"/>
        <rdfs:label xml:lang="en">CableCar</rdfs:label>
    </owl:NamedIndividual>
    


    <!-- https://w3id.org/transmodel/journeys#CorridorService -->

    <owl:NamedIndividual rdf:about="https://w3id.org/transmodel/journeys#CorridorService">
        <rdfs:label xml:lang="en">CorridorService</rdfs:label>
    </owl:NamedIndividual>
    


    <!-- https://w3id.org/transmodel/journeys#DefaultInterchangeMaximum -->

    <owl:NamedIndividual rdf:about="https://w3id.org/transmodel/journeys#DefaultInterchangeMaximum">
        <rdf:type rdf:resource="https://w3id.org/transmodel/journeys#DefaultInterchange"/>
        <rdfs:label xml:lang="en">DefaultInterchangeStandard</rdfs:label>
    </owl:NamedIndividual>
    


    <!-- https://w3id.org/transmodel/journeys#DefaultInterchangeStandard -->

    <owl:NamedIndividual rdf:about="https://w3id.org/transmodel/journeys#DefaultInterchangeStandard">
        <rdf:type rdf:resource="https://w3id.org/transmodel/journeys#DefaultInterchange"/>
        <rdfs:label xml:lang="en">DefaultInterchangeMaximum</rdfs:label>
    </owl:NamedIndividual>
    


    <!-- https://w3id.org/transmodel/journeys#Ferry -->

    <owl:NamedIndividual rdf:about="https://w3id.org/transmodel/journeys#Ferry">
        <rdf:type rdf:resource="https://w3id.org/transmodel/journeys#MeanOfTransport"/>
        <rdfs:label xml:lang="en">Ferry</rdfs:label>
    </owl:NamedIndividual>
    


    <!-- https://w3id.org/transmodel/journeys#FixedStopAreaWideFlexibleService -->

    <owl:NamedIndividual rdf:about="https://w3id.org/transmodel/journeys#FixedStopAreaWideFlexibleService">
        <rdfs:label xml:lang="en">FixedStopAreaWideFlexibleService</rdfs:label>
    </owl:NamedIndividual>
    


    <!-- https://w3id.org/transmodel/journeys#FlexibleServiceWithMainRoute -->

    <owl:NamedIndividual rdf:about="https://w3id.org/transmodel/journeys#FlexibleServiceWithMainRoute">
        <rdfs:label xml:lang="en">FlexibleServiceWithMainRoute</rdfs:label>
    </owl:NamedIndividual>
    


    <!-- https://w3id.org/transmodel/journeys#FreeAreaWideFlexibleService -->

    <owl:NamedIndividual rdf:about="https://w3id.org/transmodel/journeys#FreeAreaWideFlexibleService">
        <rdfs:label xml:lang="en">FreeAreaWideFlexibleService</rdfs:label>
    </owl:NamedIndividual>
    


    <!-- https://w3id.org/transmodel/journeys#Friday -->

    <owl:NamedIndividual rdf:about="https://w3id.org/transmodel/journeys#Friday">
        <rdfs:label xml:lang="en">Friday</rdfs:label>
    </owl:NamedIndividual>
    


    <!-- https://w3id.org/transmodel/journeys#FromOriginToSSP -->

    <owl:NamedIndividual rdf:about="https://w3id.org/transmodel/journeys#FromOriginToSSP">
        <rdf:type rdf:resource="https://w3id.org/transmodel/journeys#Access"/>
    </owl:NamedIndividual>
    


    <!-- https://w3id.org/transmodel/journeys#FromSSPtoDestination -->

    <owl:NamedIndividual rdf:about="https://w3id.org/transmodel/journeys#FromSSPtoDestination">
        <rdf:type rdf:resource="https://w3id.org/transmodel/journeys#Access"/>
    </owl:NamedIndividual>
    


    <!-- https://w3id.org/transmodel/journeys#Funicular -->

    <owl:NamedIndividual rdf:about="https://w3id.org/transmodel/journeys#Funicular">
        <rdf:type rdf:resource="https://w3id.org/transmodel/journeys#MeanOfTransport"/>
        <rdfs:label xml:lang="en">Funicular</rdfs:label>
    </owl:NamedIndividual>
    


    <!-- https://w3id.org/transmodel/journeys#Gondola -->

    <owl:NamedIndividual rdf:about="https://w3id.org/transmodel/journeys#Gondola">
        <rdf:type rdf:resource="https://w3id.org/transmodel/journeys#MeanOfTransport"/>
        <rdfs:label xml:lang="en">Gondola</rdfs:label>
    </owl:NamedIndividual>
    


    <!-- https://w3id.org/transmodel/journeys#Metro -->

    <owl:NamedIndividual rdf:about="https://w3id.org/transmodel/journeys#Metro">
        <rdf:type rdf:resource="https://w3id.org/transmodel/journeys#MeanOfTransport"/>
        <rdfs:label xml:lang="en">Metro</rdfs:label>
    </owl:NamedIndividual>
    


    <!-- https://w3id.org/transmodel/journeys#MixedTypeOfFlexibleAndRegularServices -->

    <owl:NamedIndividual rdf:about="https://w3id.org/transmodel/journeys#MixedTypeOfFlexibleAndRegularServices">
        <rdfs:label xml:lang="en">MixedTypeOfFlexibleAndRegularServices</rdfs:label>
    </owl:NamedIndividual>
    


    <!-- https://w3id.org/transmodel/journeys#MixedTypesOfFlexibleService -->

    <owl:NamedIndividual rdf:about="https://w3id.org/transmodel/journeys#MixedTypesOfFlexibleService">
        <rdfs:label xml:lang="en">MixedTypesOfFlexibleService</rdfs:label>
    </owl:NamedIndividual>
    


    <!-- https://w3id.org/transmodel/journeys#Monday -->

    <owl:NamedIndividual rdf:about="https://w3id.org/transmodel/journeys#Monday">
        <rdfs:label xml:lang="en">Monday</rdfs:label>
    </owl:NamedIndividual>
    


    <!-- https://w3id.org/transmodel/journeys#OneDirection -->

    <owl:NamedIndividual rdf:about="https://w3id.org/transmodel/journeys#OneDirection">
        <rdf:type rdf:resource="https://w3id.org/transmodel/journeys#AllowedLineDirections"/>
        <rdfs:label xml:lang="en">OneDirection</rdfs:label>
    </owl:NamedIndividual>
    


    <!-- https://w3id.org/transmodel/journeys#OtherDirections -->

    <owl:NamedIndividual rdf:about="https://w3id.org/transmodel/journeys#OtherDirections">
        <rdf:type rdf:resource="https://w3id.org/transmodel/journeys#AllowedLineDirections"/>
        <rdfs:label xml:lang="en">OtherDirections</rdfs:label>
    </owl:NamedIndividual>
    


    <!-- https://w3id.org/transmodel/journeys#OutboundRoute -->

    <owl:NamedIndividual rdf:about="https://w3id.org/transmodel/journeys#OutboundRoute">
        <rdfs:label xml:lang="en">Outbound</rdfs:label>
    </owl:NamedIndividual>
    


    <!-- https://w3id.org/transmodel/journeys#PrivateBike -->

    <owl:NamedIndividual rdf:about="https://w3id.org/transmodel/journeys#PrivateBike">
        <rdf:type rdf:resource="https://w3id.org/transmodel/journeys#AccessMode"/>
    </owl:NamedIndividual>
    


    <!-- https://w3id.org/transmodel/journeys#Rail -->

    <owl:NamedIndividual rdf:about="https://w3id.org/transmodel/journeys#Rail">
        <rdf:type rdf:resource="https://w3id.org/transmodel/journeys#MeanOfTransport"/>
        <rdfs:label xml:lang="en">Rail</rdfs:label>
    </owl:NamedIndividual>
    


    <!-- https://w3id.org/transmodel/journeys#ReturnRoute -->

    <owl:NamedIndividual rdf:about="https://w3id.org/transmodel/journeys#ReturnRoute">
        <rdfs:label xml:lang="en">ReturnRoute</rdfs:label>
    </owl:NamedIndividual>
    


    <!-- https://w3id.org/transmodel/journeys#RoundTrip -->

    <owl:NamedIndividual rdf:about="https://w3id.org/transmodel/journeys#RoundTrip">
        <rdfs:label xml:lang="en">RoundTrip</rdfs:label>
    </owl:NamedIndividual>
    


    <!-- https://w3id.org/transmodel/journeys#Saturday -->

    <owl:NamedIndividual rdf:about="https://w3id.org/transmodel/journeys#Saturday">
        <rdfs:label xml:lang="en">Saturday</rdfs:label>
    </owl:NamedIndividual>
    


    <!-- https://w3id.org/transmodel/journeys#Sunday -->

    <owl:NamedIndividual rdf:about="https://w3id.org/transmodel/journeys#Sunday">
        <rdfs:label xml:lang="en">Sunday</rdfs:label>
    </owl:NamedIndividual>
    


    <!-- https://w3id.org/transmodel/journeys#Thursday -->

    <owl:NamedIndividual rdf:about="https://w3id.org/transmodel/journeys#Thursday">
        <rdfs:label xml:lang="en">Thursday</rdfs:label>
    </owl:NamedIndividual>
    


    <!-- https://w3id.org/transmodel/journeys#Tram -->

    <owl:NamedIndividual rdf:about="https://w3id.org/transmodel/journeys#Tram">
        <rdf:type rdf:resource="https://w3id.org/transmodel/journeys#MeanOfTransport"/>
        <rdfs:label xml:lang="en">Tram</rdfs:label>
    </owl:NamedIndividual>
    


    <!-- https://w3id.org/transmodel/journeys#Tuesday -->

    <owl:NamedIndividual rdf:about="https://w3id.org/transmodel/journeys#Tuesday">
        <rdfs:label xml:lang="en">Tuesday</rdfs:label>
    </owl:NamedIndividual>
    


    <!-- https://w3id.org/transmodel/journeys#Walking -->

    <owl:NamedIndividual rdf:about="https://w3id.org/transmodel/journeys#Walking">
        <rdf:type rdf:resource="https://w3id.org/transmodel/journeys#AccessMode"/>
    </owl:NamedIndividual>
    


    <!-- https://w3id.org/transmodel/journeys#Wednesday -->

    <owl:NamedIndividual rdf:about="https://w3id.org/transmodel/journeys#Wednesday">
        <rdfs:label xml:lang="en">Wednesday</rdfs:label>
    </owl:NamedIndividual>
    


    <!-- https://w3id.org/transmodel/journeys#WeekdayInSchoolHolidays -->

    <owl:NamedIndividual rdf:about="https://w3id.org/transmodel/journeys#WeekdayInSchoolHolidays">
        <rdfs:label xml:lang="en">WeekdayInSchoolHolidays</rdfs:label>
    </owl:NamedIndividual>
    


    <!-- https://w3id.org/transmodel/journeys#virtualLineService -->

    <owl:NamedIndividual rdf:about="https://w3id.org/transmodel/journeys#virtualLineService">
        <rdfs:label xml:lang="en">VirtualLineService</rdfs:label>
    </owl:NamedIndividual>
    


    <!-- https://w3id.org/transmodel/kos/commons/all-modes -->

    <owl:NamedIndividual rdf:about="https://w3id.org/transmodel/kos/commons/all-modes">
        <rdf:type rdf:resource="http://www.w3.org/2004/02/skos/core#ConceptScheme"/>
    </owl:NamedIndividual>
    


    <!-- https://w3id.org/transmodel/kos/journeys/day-type -->

    <owl:NamedIndividual rdf:about="https://w3id.org/transmodel/kos/journeys/day-type">
        <rdf:type rdf:resource="http://www.w3.org/2004/02/skos/core#ConceptScheme"/>
        <rdfs:comment xml:lang="en">Concept scheme where all the codelists for the types of datatype properties that are included in the Transmodel ontology</rdfs:comment>
        <rdfs:comment xml:lang="en">TODO: determine whether there may be split into serveral kos or not</rdfs:comment>
        <rdfs:label xml:lang="en">day type</rdfs:label>
    </owl:NamedIndividual>
    


    <!-- https://w3id.org/transmodel/kos/journeys/direction-type -->

    <owl:NamedIndividual rdf:about="https://w3id.org/transmodel/kos/journeys/direction-type">
        <rdf:type rdf:resource="http://www.w3.org/2004/02/skos/core#ConceptScheme"/>
        <rdfs:comment xml:lang="en">Concept scheme for types of directions (inbound, outbound, clockwise, anticlockwise)</rdfs:comment>
    </owl:NamedIndividual>
    


    <!-- https://w3id.org/transmodel/kos/journeys/entrance-type -->

    <owl:NamedIndividual rdf:about="https://w3id.org/transmodel/kos/journeys/entrance-type">
        <rdf:type rdf:resource="http://www.w3.org/2004/02/skos/core#ConceptScheme"/>
        <rdfs:comment xml:lang="en">Concept scheme where all the codelists for the types of entrance types that are included in the Transmodel ontology</rdfs:comment>
    </owl:NamedIndividual>
    


    <!-- https://w3id.org/transmodel/kos/journeys/interchange-weighting-type -->

    <owl:NamedIndividual rdf:about="https://w3id.org/transmodel/kos/journeys/interchange-weighting-type">
        <rdf:type rdf:resource="http://www.w3.org/2004/02/skos/core#ConceptScheme"/>
        <rdfs:comment xml:lang="en">Concept scheme where all the codelists for the types of interchange weighting types that are included in the Transmodel ontology</rdfs:comment>
    </owl:NamedIndividual>
    


    <!-- https://w3id.org/transmodel/kos/journeys/limited-use-type -->

    <owl:NamedIndividual rdf:about="https://w3id.org/transmodel/kos/journeys/limited-use-type">
        <rdf:type rdf:resource="http://www.w3.org/2004/02/skos/core#ConceptScheme"/>
        <rdfs:comment xml:lang="en">Concept scheme where all the codelists for the types of limited use that are included in the Transmodel ontology</rdfs:comment>
    </owl:NamedIndividual>
    


    <!-- https://w3id.org/transmodel/kos/journeys/mobility-limitation -->

    <owl:NamedIndividual rdf:about="https://w3id.org/transmodel/kos/journeys/mobility-limitation">
        <rdf:type rdf:resource="http://www.w3.org/2004/02/skos/core#ConceptScheme"/>
        <rdfs:comment xml:lang="en">Concept scheme  for types of mobility limitations</rdfs:comment>
        <rdfs:label xml:lang="en">mobility-limitation</rdfs:label>
    </owl:NamedIndividual>
    


    <!-- https://w3id.org/transmodel/kos/journeys/quay-type -->

    <owl:NamedIndividual rdf:about="https://w3id.org/transmodel/kos/journeys/quay-type">
        <rdf:type rdf:resource="http://www.w3.org/2004/02/skos/core#ConceptScheme"/>
        <rdfs:comment xml:lang="en">Concept scheme where all the codelists for the types of quay types that are included in the Transmodel ontology</rdfs:comment>
    </owl:NamedIndividual>
    


    <!-- https://w3id.org/transmodel/kos/journeys/stop-place -->

    <owl:NamedIndividual rdf:about="https://w3id.org/transmodel/kos/journeys/stop-place">
        <rdf:type rdf:resource="http://www.w3.org/2004/02/skos/core#ConceptScheme"/>
        <rdfs:comment xml:lang="en">Concept scheme  for types of stop place</rdfs:comment>
        <rdfs:label xml:lang="en">stop-place</rdfs:label>
    </owl:NamedIndividual>
    


    <!-- https://w3id.org/transmodel/kos/journeys/stop-place-component-type -->

    <owl:NamedIndividual rdf:about="https://w3id.org/transmodel/kos/journeys/stop-place-component-type">
        <rdf:type rdf:resource="http://www.w3.org/2004/02/skos/core#ConceptScheme"/>
        <rdfs:comment xml:lang="en">Concept scheme where all the codelists for the types of stop place component types that are included in the Transmodel ontology</rdfs:comment>
    </owl:NamedIndividual>
    


    <!-- https://w3id.org/transmodel/kos/journeys/stop-use-type -->

    <owl:NamedIndividual rdf:about="https://w3id.org/transmodel/kos/journeys/stop-use-type">
        <rdf:type rdf:resource="http://www.w3.org/2004/02/skos/core#ConceptScheme"/>
        <rdfs:comment xml:lang="en">Concept scheme  for types of use of stops (e.g., access, interchange only, pass through or non boarding alighting)</rdfs:comment>
        <rdfs:label xml:lang="en">stop-use-type</rdfs:label>
    </owl:NamedIndividual>
    <rdf:Description>
        <mbox xml:lang="en">adolfo.anton.bravo@upm.es</mbox>
        <name xml:lang="en">Adolfo Anton-Bravo</name>
    </rdf:Description>
    


    <!-- 
    ///////////////////////////////////////////////////////////////////////////////////////
    //
    // Annotations
    //
    ///////////////////////////////////////////////////////////////////////////////////////
     -->

    <rdf:Description rdf:about="https://w3id.org/transmodel/journeys#timingLinkInJourneyPattern">
        <rdfs:label xml:lang="en">timingLinkInJourneyPattern</rdfs:label>
    </rdf:Description>
</rdf:RDF>



<!-- Generated by the OWL API (version 4.5.9.2019-02-01T07:24:44Z) https://github.com/owlcs/owlapi -->
